doc/coq/signature/ConcretEquivalence.v
@@ -1,0 +1,2601 @@
+From Signature Require Export Bound.
+
+Generalizable Variables T TT aT aTT.
+
+Lemma capp_nil_r {T} :
+  forall (C : dy_ctx T), C [|([||])|] = C.
+Proof.
+  induction C; ii; ss; rw; exact eq_refl.
+Qed.
+
+Lemma app_same `{Eq T} :
+  forall l l' m m'
+    (SAMEl : same l l')
+    (SAMEm : same m m'),
+    same (l ++ m) (l' ++ m').
+Proof.
+  pose proof read_top.
+  ii. repeat rw. unfold same in SAMEl.
+  repeat des_goal; clarify;
+  repeat match goal with
+  | H : read _ _ = _ |- _ => symmetry in H
+  end;
+  first [rewrite SAMEl in * | rewrite <- SAMEl in *];
+  match goal with
+  | _ : ?a = read ?l ?t, _ : ?b = read ?l ?t |- _ =>
+    assert (a = b); clarify; repeat rw; eauto
+  end.
+Qed.
+
+Lemma disj_reflect `{Eq T} :
+  forall m m',
+  (forall t (READ : None <> read m t), None = read m' t) <->
+  (forall t (READ : None <> read m' t), None = read m t).
+Proof.
+  induction m; ii; ss;
+  repeat des_goal; clarify.
+  split; intros IN ? ?; try des_goal; try des_hyp; clarify.
+  - rewrite eqb_eq in *; clarify.
+    exfalso. apply READ. apply IN. rewrite t_refl.
+    red; ii; clarify.
+  - assert (forall t, None <> read m' t -> None = read m t); eauto.
+    rewrite <- IHm.
+    ii. apply IN. red; ii; des_hyp; clarify.
+  - rewrite eqb_eq in *; clarify.
+    specialize (IN t0). rewrite t_refl in *.
+    destruct (read m' t0); eauto.
+    assert (None = Some e); clarify.
+    apply IN; red; ii; clarify.
+  - assert (forall t, None <> read m t -> None = read m' t); eauto.
+    rewrite IHm.
+    ii. specialize (IN t1). apply IN in READ0.
+    des_hyp; clarify.
+Qed.
+
+Lemma app_disj_same `{Eq T} :
+  forall m m' (DISJ : forall t (READ : None <> read m t), None = read m' t),
+  same (m ++ m') (m' ++ m).
+Proof.
+  induction m; ii; ss.
+  - rewrite app_nil_r. eauto.
+  - des_goal.
+    assert (None = read m' t0).
+    apply DISJ. rewrite t_refl. red; ii; clarify.
+    des_goal; clarify.
+    + rewrite eqb_eq in *; clarify.
+      clear IHm DISJ.
+      ginduction m'; ii; ss. rewrite t_refl. eauto.
+      repeat des_hyp; clarify; eauto.
+    + assert (read (m' ++ (t0, e) :: m) t = read (m' ++ m) t) as RR.
+      {
+        clear H0 v DISJ IHm.
+        ginduction m'; ii; ss. rw. eauto.
+        repeat des_goal; clarify; eauto.
+      }
+      rewrite RR.
+      apply IHm. ii. apply DISJ.
+      red; ii. repeat des_hyp; clarify.
+Qed.
+
+Lemma eq_root_neq `{Eq T} :
+  forall r r', eq_root r r' = false <-> r <> r'.
+Proof.
+  assert (eq_root = eqb) as RR. reflexivity.
+  rewrite RR in *. exact eqb_neq.
+Qed.
+
+Lemma same_comm `{Eq T} :
+  forall m m',
+  same m m' <-> same m' m.
+Proof.
+  intros; unfold same; split; ii; rw; eauto.
+Qed.
+
+Lemma same_trans `{Eq T} :
+  forall m m' m'' (SAME : same m m') (SAME' : same m' m''),
+  same m m''.
+Proof.
+  ii. unfold same in *. rewrite SAME. rewrite SAME'. eauto.
+Qed.
+
+Lemma asame_comm `{Eq T} :
+  forall m m',
+  asame m m' <-> asame m' m.
+Proof.
+  intros; unfold asame; split; ii; rw; eauto.
+Qed.
+
+Lemma asame_trans `{Eq T} :
+  forall m m' m'' (SAME : asame m m') (SAME' : asame m' m''),
+  asame m m''.
+Proof.
+  ii. unfold asame in *. rewrite SAME. rewrite SAME'. eauto.
+Qed.
+
+Fixpoint remove_x `{Eq T} (C : dy_ctx T) x :=
+  match C with
+  | [||] => [||]
+  | dy_binde x' tx C =>
+    if eqb x x'
+    then remove_x C x
+    else dy_binde x' tx (remove_x C x)
+  | dy_bindm M CM C =>
+    dy_bindm M CM (remove_x C x)
+  end.
+
+Fixpoint remove_M `{Eq T} (C : dy_ctx T) M :=
+  match C with
+  | [||] => [||]
+  | dy_binde x tx C =>
+    dy_binde x tx (remove_M C M)
+  | dy_bindm M' CM C =>
+    if eqb M M'
+    then remove_M C M
+    else dy_bindm M' CM (remove_M C M)
+  end.
+
+Lemma remove_x_read_none `{Eq T} :
+  forall C x, addr_x (remove_x C x) x = None.
+Proof.
+  induction C; ii; ss.
+  repeat des_goal; eauto. clarify.
+Qed.
+
+Lemma remove_x_read_some `{Eq T} :
+  forall C x x' (NEQ : x <> x'),
+    addr_x (remove_x C x) x' = addr_x C x'.
+Proof.
+  induction C; ii; ss; eauto.
+  repeat des_goal; eauto.
+  rewrite eqb_ID_eq in *; clarify.
+Qed.
+
+Lemma remove_x_ctx `{Eq T} :
+  forall C x M,
+    ctx_M (remove_x C x) M = ctx_M C M.
+Proof.
+  induction C; ii; ss;
+  repeat des_goal; clarify.
+Qed.
+
+Lemma remove_M_read_none `{Eq T} :
+  forall C M, ctx_M (remove_M C M) M = None.
+Proof.
+  induction C; ii; ss.
+  repeat des_goal; eauto. clarify.
+Qed.
+
+Lemma remove_M_read_some `{Eq T} :
+  forall C M M' (NEQ : M <> M'),
+    ctx_M (remove_M C M) M' = ctx_M C M'.
+Proof.
+  induction C; ii; ss; eauto.
+  repeat des_goal; eauto.
+  rewrite eqb_ID_eq in *; clarify.
+Qed.
+
+Lemma remove_M_addr `{Eq T} :
+  forall C M x,
+    addr_x (remove_M C M) x = addr_x C x.
+Proof.
+  induction C; ii; ss;
+  repeat des_goal; clarify.
+Qed.
+
+Fixpoint read_fst `{Eq T} `{Eq TT}
+  (ϕ : list (T * TT)) (t : T) :=
+  match ϕ with
+  | [] => None
+  | (t', t'') :: tl =>
+    if eqb t t' then Some t'' else read_fst tl t
+  end.
+
+Fixpoint read_snd `{Eq T} `{Eq TT}
+  (ϕ : list (T * TT)) (t : TT) :=
+  match ϕ with
+  | [] => None
+  | (t'', t') :: tl =>
+    if eqb t t' then Some t'' else read_snd tl t
+  end.
+
+Lemma read_fst_top `{Eq T} `{Eq TT} :
+  forall (a b : list (T * TT)) t,
+  read_fst (a ++ b) t = 
+  match read_fst a t with
+  | None => read_fst b t
+  | Some _ => read_fst a t
+  end.
+Proof.
+  induction a; ii; ss;
+  repeat des_goal; repeat des_hyp; clarify;
+  repeat rw; reflexivity.
+Qed.
+
+Lemma read_snd_top `{Eq T} `{Eq TT} :
+  forall (a b : list (T * TT)) t,
+  read_snd (a ++ b) t = 
+  match read_snd a t with
+  | None => read_snd b t
+  | Some _ => read_snd a t
+  end.
+Proof.
+  induction a; ii; ss;
+  repeat des_goal; repeat des_hyp; clarify;
+  repeat rw; reflexivity.
+Qed.
+
+Fixpoint check_iso `{Eq T} `{Eq TT}
+  (C' : dy_ctx TT) φ φ' (Cout Cin : dy_ctx T) :=
+  match Cin with
+  | [||] => if eqb C' ([||]) then true else false
+  | dy_binde x tx Cin =>
+    match addr_x Cout x with (* is it shadowed? *)
+    | Some _ => check_iso C' φ φ' Cout Cin
+    | None =>
+      let Cout := dy_binde x tx Cout in
+      match addr_x C' x with
+      | Some tx' =>
+        if eqb (φ tx) tx' && eqb tx (φ' tx') then
+          check_iso (remove_x C' x) φ φ' Cout Cin
+        else false
+      | None => false
+      end
+    end
+  | dy_bindm M CM Cin =>
+    match ctx_M Cout M with (* is it shadowed? *)
+    | Some _ => check_iso C' φ φ' Cout Cin
+    | None =>
+      let Cout := dy_bindm M CM Cout in
+      match ctx_M C' M with
+      | Some CM' =>
+        if check_iso CM' φ φ' ([||]) CM then
+          check_iso (remove_M C' M) φ φ' Cout Cin
+        else false
+      | None => false
+      end
+    end
+  end.
+
+Definition check_iso_spec `{Eq T} `{Eq TT}
+  (C' : dy_ctx TT) φ φ' (Cout Cin : dy_ctx T) :=
+  (forall x (VIS : addr_x Cout x = None) tx p
+    (VALp : valid_path (Ctx Cin) [] (Px x tx p)),
+    let p' := pmap φ p in
+    valid_path (Ctx C') [] (Px x (φ tx) p') /\
+    φ' (φ tx) = tx /\ p = pmap φ' p') /\
+  (forall M (VIS : ctx_M Cout M = None) p
+    (VALp : valid_path (Ctx Cin) [] (PM M p)),
+    let p' := pmap φ p in
+    valid_path (Ctx C') [] (PM M p') /\
+    p = pmap φ' p') /\
+  (forall x (VIS : addr_x Cout x = None) tx' p'
+    (VALp' : valid_path (Ctx C') [] (Px x tx' p')),
+    let p := pmap φ' p' in
+    valid_path (Ctx Cin) [] (Px x (φ' tx') p) /\
+    φ (φ' tx') = tx' /\ p' = pmap φ p) /\
+  (forall M (VIS : ctx_M Cout M = None) p'
+    (VALp' : valid_path (Ctx C') [] (PM M p')),
+    let p := pmap φ' p' in
+    valid_path (Ctx Cin) [] (PM M p) /\
+    p' = pmap φ p).
+
+Definition check_aiso_spec `{Eq T} `{Eq TT}
+  (C' : dy_ctx TT) φ φ' (Cout Cin : dy_ctx T) :=
+  (forall x (VIS : addr_x Cout x = None) tx p
+    (VALp : avalid_path (Ctx Cin) [] (Px x tx p)),
+    let p' := pmap φ p in
+    avalid_path (Ctx C') [] (Px x (φ tx) p') /\
+    φ' (φ tx) = tx /\ p = pmap φ' p') /\
+  (forall M (VIS : ctx_M Cout M = None) p
+    (VALp : avalid_path (Ctx Cin) [] (PM M p)),
+    let p' := pmap φ p in
+    avalid_path (Ctx C') [] (PM M p') /\
+    p = pmap φ' p') /\
+  (forall x (VIS : addr_x Cout x = None) tx' p'
+    (VALp' : avalid_path (Ctx C') [] (Px x tx' p')),
+    let p := pmap φ' p' in
+    avalid_path (Ctx Cin) [] (Px x (φ' tx') p) /\
+    φ (φ' tx') = tx' /\ p' = pmap φ p) /\
+  (forall M (VIS : ctx_M Cout M = None) p'
+    (VALp' : avalid_path (Ctx C') [] (PM M p')),
+    let p := pmap φ' p' in
+    avalid_path (Ctx Cin) [] (PM M p) /\
+    p' = pmap φ p).
+
+Lemma check_iso_spec_true `{Eq T} `{Eq TT} :
+  forall (C' : dy_ctx TT) φ φ' (Cout Cin : dy_ctx T)
+  (PREx : forall x, addr_x Cout x <> None -> addr_x C' x = None)
+  (PREM : forall M, ctx_M Cout M <> None -> ctx_M C' M = None),
+  check_iso C' φ φ' Cout Cin = true <->
+  check_iso_spec C' φ φ' Cout Cin.
+Proof.
+  ii. split; intros ISO.
+  - ginduction Cin; ii; ss; repeat des_hyp; des; clarify.
+    + rewrite eqb_C_eq in *. clarify.
+    + apply IHCin in ISO; eauto.
+      unfold check_iso_spec in *. des.
+      split. ii; ss.
+      exploit ISO; eauto.
+      repeat des_hyp; des; clarify.
+      rewrite eqb_ID_eq in *. clarify.
+      rw. eauto.
+      split. eauto.
+      split; eauto. ii; ss.
+      exploit ISO1; eauto.
+      ii. repeat des_goal; repeat des_hyp; des; clarify.
+      rewrite eqb_ID_eq in *. clarify.
+    + repeat rewrite eqb_eq in *. clarify.
+      apply IHCin in ISO.
+      unfold check_iso_spec in *. des.
+      split. ii; ss.
+      repeat des_hyp; des; clarify.
+      rewrite eqb_ID_eq in *. clarify.
+      rw. destruct p; ss; des; clarify.
+      exploit ISO; eauto. rw. eauto. rw. eauto.
+      rewrite remove_x_read_some. eauto.
+      rewrite eqb_ID_neq in *. eauto.
+      split. ii; ss.
+      exploit ISO0; eauto.
+      rewrite remove_x_ctx. eauto.
+      split. ii; ss.
+      des_goal; repeat des_hyp; des; clarify;
+      match goal with
+      | _ : eqb_ID _ _ = true |- _ =>
+        rewrite eqb_ID_eq in *; clarify; rrw;
+        destruct p'; ss; des; clarify
+      | _ =>
+        exploit ISO1; try rw; eauto;
+        rewrite remove_x_read_some; try rw; eauto;
+        rewrite eqb_ID_neq in *; eauto
+      end.
+      ii; ss. des_hyp; clarify.
+      exploit ISO2; eauto.
+      rewrite remove_x_ctx. rw. eauto.
+      ii; ss. repeat des_hyp; clarify.
+      rewrite eqb_ID_eq in *. clarify.
+      apply remove_x_read_none.
+      rewrite remove_x_read_some. eauto.
+      rewrite eqb_ID_neq in *. eauto.
+      ii; ss. rewrite remove_x_ctx. eauto.
+    + apply IHCin2 in ISO; eauto.
+      unfold check_iso_spec in *. des.
+      split. eauto.
+      split. ii. ss.
+      repeat des_hyp; clarify.
+      rewrite eqb_ID_eq in *; clarify.
+      exploit ISO0; eauto. rw. eauto.
+      split. eauto.
+      ii. ss.
+      repeat des_hyp; clarify.
+      exploit ISO2; eauto. rw. eauto.
+      ii. repeat des_hyp; des; clarify.
+      split; eauto.
+      des_goal; repeat des_hyp; clarify.
+      rewrite eqb_ID_eq in *; clarify.
+    + match goal with 
+      | H : _ |- _ =>
+        let ISO := fresh "ISO'" in
+        apply IHCin1 in H;
+        first [solve [ii; ss] | rename H into ISO]
+      end.
+      apply IHCin2 in ISO. clear IHCin1 IHCin2.
+      unfold check_iso_spec in *. des.
+      split. ii. ss.
+      exploit ISO; eauto. ii.
+      rewrite remove_M_addr in *. eauto.
+      split. ii. ss.
+      repeat des_hyp; clarify.
+      rewrite eqb_ID_eq in *. clarify. rw.
+      destruct p; ss.
+      exploit ISO'; eauto.
+      ii; des; clarify. rw. rrw. eauto.
+      exploit ISO'0; eauto.
+      ii; des; clarify. rrw. eauto.
+      exploit ISO0; eauto.
+      rw. eauto. rw. eauto.
+      rewrite remove_M_read_some. eauto.
+      rewrite eqb_ID_neq in *. eauto.
+      split. ii; ss.
+      exploit ISO1; eauto.
+      rewrite remove_M_addr. eauto.
+      ii; ss.
+      des_goal; repeat des_hyp; clarify;
+      match goal with
+      | _ : eqb_ID _ _ = true |- _ =>
+        rewrite eqb_ID_eq in *; clarify;
+        destruct p'; ss;
+        match goal with
+        | |- context [addr_x] =>
+          exploit ISO'1; eauto;
+          ii; repeat des_hyp; des; clarify;
+          rw; rrw; eauto
+        | |- context [ctx_M] =>
+          exploit ISO'2; eauto;
+          ii; repeat des_hyp; des; clarify;
+          rrw; eauto
+        end
+      | _ : eqb_ID _ _ = false |- _ =>
+        exploit ISO2; eauto;
+        repeat match goal with
+        | _ => rw
+        | _ => solve [eauto]
+        | _ => rewrite remove_M_read_some
+        | _ => rewrite eqb_ID_neq in *
+        end
+      end.
+      ii; ss. rewrite remove_M_addr. eauto.
+      ii; ss. des_hyp; clarify.
+      rewrite eqb_ID_eq in *. clarify.
+      rewrite remove_M_read_none. eauto.
+      rewrite remove_M_read_some. eauto.
+      rewrite eqb_ID_neq in *. eauto.
+  - ginduction Cin; ii; ss; clarify.
+    assert (forall x, addr_x C' x = None) as contrax.
+    {
+      ii. destruct (addr_x Cout x) eqn:CASE.
+      apply PREx. rw. ss.
+      unfold check_iso_spec in *. des.
+      destruct (addr_x C' x) eqn:CASE'; eauto.
+      exploit ISO1; eauto. ss. rw. split. reflexivity.
+      instantiate (1 := Pnil). ss.
+      ii; des; ss.
+    }
+    assert (forall M, ctx_M C' M = None) as contraM.
+    {
+      ii. destruct (ctx_M Cout M) eqn:CASE.
+      apply PREM. rw. ss.
+      unfold check_iso_spec in *. des.
+      destruct (ctx_M C' M) eqn:CASE'; eauto.
+      exploit ISO2; eauto. ss. rw.
+      instantiate (1 := Pnil). ss.
+      ii; des; ss.
+    }
+    assert (C' = [||]) as RR.
+    {
+      destruct C'; ss.
+      specialize (contrax x). rewrite ID_refl in *. clarify.
+      specialize (contraM M). rewrite ID_refl in *. clarify.
+    }
+    rewrite RR. assert (eqb_C = eqb) as RR'. eauto.
+    rewrite RR'. rewrite t_refl. eauto.
+    + repeat des_goal; unfold check_iso_spec in *; des.
+      apply IHCin; eauto.
+      split. ii; ss.
+      des_hyp; des; clarify.
+      exploit ISO; eauto. des_goal; des_hyp; clarify.
+      rewrite eqb_ID_eq in *. clarify.
+      split. eauto.
+      split; eauto.
+      ii. ss. des_hyp; des; clarify.
+      exploit ISO1; eauto. rw. eauto.
+      eauto. ii. repeat des_hyp; des; clarify.
+      rewrite eqb_ID_eq in *. clarify.
+      repeat rw. eauto.
+      apply IHCin; eauto.
+      ii; ss. des_hyp; clarify.
+      rewrite eqb_ID_eq in *. clarify. apply remove_x_read_none.
+      rewrite remove_x_read_some. eauto.
+      rewrite eqb_ID_neq in *. eauto.
+      ii; ss. rewrite remove_x_ctx. eauto.
+      repeat rewrite eqb_eq in *. clarify.
+      unfold check_iso_spec in *. des.
+      split. ii; ss.
+      repeat des_hyp; des; clarify.
+      exploit ISO; eauto.
+      rw. rw. eauto.
+      rewrite remove_x_read_some. eauto.
+      rewrite eqb_ID_neq in *. eauto.
+      split. ii; ss.
+      repeat des_hyp; des; clarify.
+      exploit ISO0; eauto.
+      rw. eauto. rewrite remove_x_ctx. eauto.
+      split; ii; ss; repeat des_hyp; des; clarify.
+      exploit ISO1; eauto.
+      rewrite remove_x_read_some in *.
+      rw. split; eauto. rewrite eqb_ID_neq in *. eauto.
+      rw. eauto.
+      exploit ISO2; eauto.
+      rewrite remove_x_ctx in *. rw. eauto.
+      rewrite eqb_eq in *. clarify.
+      exploit ISO1. eauto.
+      ss. rw. split. reflexivity.
+      instantiate (1 := Pnil). ss.
+      ii; des; ss. rewrite ID_refl in *.
+      des; clarify. rewrite eqb_neq in *. contradict.
+      exploit ISO1. eauto. ss. rw.
+      split. reflexivity. instantiate (1 := Pnil). ss.
+      ii; des; ss. rewrite ID_refl in *.
+      des; clarify. rewrite eqb_neq in *. contradict.
+      exploit ISO. eauto.
+      ss. rewrite ID_refl. split; eauto.
+      instantiate (1 := Pnil). ss.
+      ii; des; ss. des_hyp; clarify.
+    + repeat des_goal; unfold check_iso_spec in *; des.
+      apply IHCin2; eauto.
+      split. eauto.
+      split. ii. ss.
+      des_hyp; clarify.
+      exploit ISO0; eauto. rw.
+      des_goal; des_hyp; clarify.
+      rewrite eqb_ID_eq in *; clarify.
+      split; eauto. ii. ss.
+      des_hyp; clarify.
+      exploit ISO2; eauto. rw. eauto.
+      ii. repeat des_hyp; des; clarify.
+      rewrite eqb_ID_eq in *; clarify.
+      des_goal; clarify.
+      apply IHCin2.
+      ii; ss. rewrite remove_M_addr. eauto.
+      ii; ss. des_hyp; clarify.
+      rewrite eqb_ID_eq in *; clarify.
+      apply remove_M_read_none.
+      rewrite remove_M_read_some; eauto.
+      rewrite eqb_ID_neq in *. eauto.
+      split. ii. ss.
+      des_hyp; des; clarify.
+      rewrite remove_M_addr.
+      exploit ISO; eauto. rw. eauto.
+      split. ii; ss.
+      repeat des_hyp; clarify.
+      rewrite remove_M_read_some.
+      exploit ISO0; eauto. rw. rw. eauto.
+      rewrite eqb_ID_neq in *. eauto.
+      split; ii; ss.
+      rewrite remove_M_addr in *. eauto.
+      repeat des_hyp; clarify.
+      rewrite remove_M_read_some in *.
+      exploit ISO2; eauto. rw. eauto.
+      rw. eauto. rewrite eqb_ID_neq in *. eauto.
+      assert (iso (Ctx d) [] (Ctx Cin1) [] φ' φ) as [HINT HINT'].
+      {
+        split; ii; ss.
+        exploit (ISO2 M). eauto. rw. eauto.
+        rewrite ID_refl. subst p'. ii; des; eauto.
+        exploit (ISO0 M). eauto.
+        rewrite ID_refl. eauto. rw. subst p.
+        ii; des; eauto.
+      }
+      assert (check_iso d φ φ' ([||]) Cin1 <> true) as RR.
+      refl_bool. eauto.
+      exfalso. apply RR. apply IHCin1; try solve [ii; ss].
+      repeat first [ii;
+      solve [exploit HINT'; eauto;
+            ii; ss; des; clarify|
+            exploit HINT; eauto;
+            ii; ss; des; clarify] | split].
+      exploit ISO0. eauto. instantiate (1 := Pnil). ss.
+      rewrite ID_refl. eauto.
+      ii; des; ss. des_hyp; clarify.
+Qed.
+
+Lemma empty_then_avalid_valid `{Eq T} :
+  forall p r,
+  avalid_path r [] p <-> valid_path r [] p.
+Proof.
+  induction p; ii; ss;
+  repeat des_goal; clarify.
+  rw. eauto.
+  split; ii; des; clarify.
+Qed.
+
+Lemma check_aiso_spec_true `{Eq T} `{Eq TT} :
+  forall (C' : dy_ctx TT) φ φ' (Cout Cin : dy_ctx T)
+  (PREx : forall x, addr_x Cout x <> None -> addr_x C' x = None)
+  (PREM : forall M, ctx_M Cout M <> None -> ctx_M C' M = None),
+  check_iso C' φ φ' Cout Cin = true <->
+  check_aiso_spec C' φ φ' Cout Cin.
+Proof.
+  ii. pose proof (check_iso_spec_true C' φ φ' Cout Cin PREx PREM) as RR.
+  rewrite RR. clear RR.
+  split; intros ISO;
+  unfold check_iso_spec in *;
+  unfold check_aiso_spec in *;
+  des.
+  - split. ii. exploit (ISO x VIS tx p);
+    rewrite empty_then_avalid_valid in *; eauto.
+    split. ii. exploit (ISO0 M VIS p);
+    rewrite empty_then_avalid_valid in *; eauto.
+    split. ii. exploit (ISO1 x VIS tx' p');
+    rewrite empty_then_avalid_valid in *; eauto.
+    ii. exploit (ISO2 M VIS p');
+    rewrite empty_then_avalid_valid in *; eauto.
+  - split. ii. exploit (ISO x VIS tx p);
+    rewrite empty_then_avalid_valid in *; eauto.
+    split. ii. exploit (ISO0 M VIS p);
+    rewrite empty_then_avalid_valid in *; eauto.
+    split. ii. exploit (ISO1 x VIS tx' p');
+    rewrite empty_then_avalid_valid in *; eauto.
+    ii. exploit (ISO2 M VIS p');
+    rewrite empty_then_avalid_valid in *; eauto.
+Qed.
+
+Definition iso_C `{Eq T} `{Eq TT} 
+  (C : dy_ctx T) (C' :dy_ctx TT) φ φ' := 
+  check_iso C' φ φ' ([||]) C
+.
+
+Lemma check_iso_iso `{Eq T} `{Eq TT} :
+  forall (C' : dy_ctx TT) φ φ' (C : dy_ctx T),
+  iso_C C C' φ φ' = true <->
+  iso (Ctx C) [] (Ctx C') [] φ φ'.
+Proof.
+  unfold iso_C.
+  ii; split; intros ISO;
+  rewrite check_iso_spec_true in *; ii; ss.
+  - unfold check_iso_spec in *. des.
+    split. ii. subst p'. destruct p; try solve [ss].
+    exploit ISO; eauto. ii; des.
+    split; eauto. s. rrw. rw. eauto.
+    exploit ISO0; eauto. ii; des.
+    split; eauto. s. rrw. eauto.
+    ii. subst p. destruct p'; try solve [ss].
+    exploit ISO1; eauto. ii; des.
+    split; eauto. s. rrw. rw. eauto.
+    exploit ISO2; eauto. ii; des.
+    split; eauto. s. rrw. eauto.
+  - destruct ISO as [ISO ISO'].
+    repeat first [ii;
+      solve [exploit ISO; eauto; ii; ss; des; clarify
+      | exploit ISO'; eauto; ii; ss; des; clarify]
+      | split].
+Qed.
+
+Definition aiso_C `{Eq T} `{Eq TT} 
+  (C : dy_ctx T) (C' :dy_ctx TT) φ φ' := 
+  check_iso C' φ φ' ([||]) C
+.
+
+Lemma check_aiso_aiso `{Eq T} `{Eq TT} :
+  forall (C' : dy_ctx TT) φ φ' (C : dy_ctx T),
+  aiso_C C C' φ φ' = true <->
+  aiso (Ctx C) [] (Ctx C') [] φ φ'.
+Proof.
+  unfold aiso_C.
+  ii; split; intros ISO;
+  rewrite check_aiso_spec_true in *; ii; ss.
+  - unfold check_aiso_spec in *. des.
+    split. ii. subst p'. destruct p; try solve [ss].
+    exploit ISO; eauto. ii; des.
+    split; eauto. s. rrw. rw. eauto.
+    exploit ISO0; eauto. ii; des.
+    split; eauto. s. rrw. eauto.
+    ii. subst p. destruct p'; try solve [ss].
+    exploit ISO1; eauto. ii; des.
+    split; eauto. s. rrw. rw. eauto.
+    exploit ISO2; eauto. ii; des.
+    split; eauto. s. rrw. eauto.
+  - destruct ISO as [ISO ISO'].
+    repeat first [ii;
+      solve [exploit ISO; eauto; ii; ss; des; clarify
+      | exploit ISO'; eauto; ii; ss; des; clarify]
+      | split].
+Qed.
+
+Lemma iso_C_is_aiso_C `{Eq T} `{Eq TT} (C : dy_ctx T) (C' : dy_ctx TT) φ φ' :
+  iso_C C C' φ φ' = aiso_C C C' φ φ'.
+Proof. reflexivity. Qed.
+
+(* lift unreachable Cs *)
+Fixpoint lift_C `{Eq T} `{Eq aT}
+  (inv_α : (T * aT) -> T) (t : T) (C : dy_ctx aT) :=
+  match C with
+  | [||] => [||]
+  | dy_binde x tx C =>
+    let tx := inv_α (t, tx) in
+    let C := lift_C inv_α t C in
+    dy_binde x tx C
+  | dy_bindm M C_M C =>
+    let C_M := lift_C inv_α t C_M in
+    let C := lift_C inv_α t C in
+    dy_bindm M C_M C
+  end.
+
+Fixpoint trans_iso_C `{Eq TT} `{TotalOrder T} `{Eq aT} (inv_α : (T * aT) -> T)
+  (C' : dy_ctx TT) (ϕ : list (TT * T)) (t : T) (Cout : dy_ctx T) (Cin : dy_ctx aT) :=
+  match Cin with
+  | [||] => Some (Cout, ϕ, t)
+  | dy_binde x tx Cin =>
+    match addr_x Cout x with (* is it shadowed? *)
+    | Some _ =>
+      let tx := inv_α (t, tx) in
+      trans_iso_C inv_α C' ϕ t (Cout [|dy_binde x tx ([||])|]) Cin
+    | None =>
+      match addr_x C' x with
+      | Some tx' =>
+        match read_fst ϕ tx' with
+        | Some tx =>
+          trans_iso_C inv_α C' ϕ t (Cout [|dy_binde x tx ([||])|]) Cin
+        | None =>
+          let tx := inv_α (t, tx) in
+          let ϕ := (tx', tx) :: ϕ in
+          trans_iso_C inv_α C' ϕ tx (Cout [| dy_binde x tx ([||]) |]) Cin
+        end
+      | None => None
+      end
+    end
+  | dy_bindm M CM Cin =>
+    match ctx_M Cout M with (* is it shadowed? *)
+    | Some _ =>
+      let CM := lift_C inv_α t CM in
+      trans_iso_C inv_α C' ϕ t (Cout [|dy_bindm M CM ([||])|]) Cin
+    | None =>
+      match ctx_M C' M with
+      | Some CM' =>
+        match trans_iso_C inv_α CM' ϕ t ([||]) CM with
+        | Some (CM, ϕ, t) =>
+          trans_iso_C inv_α C' ϕ t (Cout [|dy_bindm M CM ([||])|]) Cin
+        | None => None
+        end
+      | None => None
+      end
+    end
+  end.
+
+Definition inv_α_spec `{TotalOrder T} `{Eq aT}
+  (α : T -> aT) (inv_α : (T * aT) -> T) :=
+  forall t abs_t,
+    t << inv_α (t, abs_t) /\
+    abs_t = α (inv_α (t, abs_t)).
+
+Lemma lift_C_lower `{TotalOrder T} `{Eq aT}
+  (α : T -> aT) inv_α (SPEC : inv_α_spec α inv_α) :
+  forall C t, trans_C α (lift_C inv_α t C) = C.  
+Proof.
+  induction C; ii; ss; repeat rw; eauto.
+  destruct (SPEC t tx). rrw. eauto.
+Qed.
+
+Definition ϕ_spec `{Eq TT} `{Eq aTT} `{TotalOrder T} `{Eq aT}
+  (α' : TT -> aTT) (α : T -> aT) (φ : aTT -> aT) (φ' : aT -> aTT)
+  (ϕ : list (TT * T)) (t : T) :=
+  forall t'' t' (IN : In (t'', t') ϕ),
+    Some t' = read_fst ϕ t'' /\
+    Some t'' = read_snd ϕ t' /\
+    leb t' t = true /\
+    α t' = φ (α' t'') /\
+    α' t'' = φ' (α t').
+
+Lemma read_fst_in `{Eq T} `{Eq TT} (ϕ : list (T * TT)) :
+  forall t t' (READ : Some t' = read_fst ϕ t),
+    In (t, t') ϕ.
+Proof.
+  induction ϕ; ii; ss; repeat des_hyp; clarify; eauto.
+  rewrite eqb_eq in *; clarify; eauto.
+Qed.
+
+Lemma in_read_fst `{Eq T} `{Eq TT} (ϕ : list (T * TT)) :
+  forall t t' (IN : In (t, t') ϕ),
+    exists t'', Some t'' = read_fst ϕ t.
+Proof.
+  induction ϕ; ii; ss; repeat des_hyp; des; clarify; eauto.
+  rewrite t_refl. eauto.
+  exploit IHϕ; eauto. ii; des; clarify.
+  repeat des_goal; clarify; eauto.
+Qed.
+
+Lemma read_snd_in `{Eq T} `{Eq TT} (ϕ : list (T * TT)) :
+  forall t t' (READ : Some t = read_snd ϕ t'),
+    In (t, t') ϕ.
+Proof.
+  induction ϕ; ii; ss; repeat des_hyp; clarify; eauto.
+  rewrite eqb_eq in *; clarify; eauto.
+Qed.
+
+Lemma in_read_snd `{Eq T} `{Eq TT} (ϕ : list (T * TT)) :
+  forall t t' (IN : In (t, t') ϕ),
+    exists t'', Some t'' = read_snd ϕ t'.
+Proof.
+  induction ϕ; ii; ss; repeat des_hyp; des; clarify; eauto.
+  rewrite t_refl. eauto.
+  exploit IHϕ; eauto. ii; des; clarify.
+  repeat des_goal; clarify; eauto.
+Qed.
+
+Fixpoint pmap_fst `{Eq T} `{Eq TT} (ϕ: list (T * TT)) (p : path T) :=
+  match p with
+  | Pnil => Some Pnil
+  | Px x tx p =>
+    match read_fst ϕ tx with
+    | Some tx =>
+      match pmap_fst ϕ p with
+      | Some p => Some (Px x tx p)
+      | None => None
+      end
+    | None => None
+    end
+  | PM M p =>
+    match pmap_fst ϕ p with
+    | Some p => Some (PM M p)
+    | None => None
+    end
+  | Pv v p =>
+    match pmap_fst ϕ p with
+    | Some p => Some (Pv v p)
+    | None => None
+    end
+  end.
+
+Fixpoint pmap_snd `{Eq T} `{Eq TT} (ϕ : list (T * TT)) (p : path TT) :=
+  match p with
+  | Pnil => Some Pnil
+  | Px x tx p =>
+    match read_snd ϕ tx with
+    | Some tx =>
+      match pmap_snd ϕ p with
+      | Some p => Some (Px x tx p)
+      | None => None
+      end
+    | None => None
+    end
+  | PM M p =>
+    match pmap_snd ϕ p with
+    | Some p => Some (PM M p)
+    | None => None
+    end
+  | Pv v p =>
+    match pmap_snd ϕ p with
+    | Some p => Some (Pv v p)
+    | None => None
+    end
+  end.
+
+Lemma pmap_ϕ_bij `{Eq T} `{Eq TT} (ϕ : list (T * TT))
+  (PRE : forall t t' (IN : In (t, t') ϕ),
+    Some t' = read_fst ϕ t /\
+    Some t = read_snd ϕ t') :
+  forall p p',
+    Some p' = pmap_fst ϕ p <-> Some p = pmap_snd ϕ p'.
+Proof.
+  assert (forall t t', In (t, t') ϕ <-> Some t' = read_fst ϕ t) as RR.
+  { ii; split; ii. exploit PRE; ii; des; eauto. apply read_fst_in; assumption. }
+  assert (forall t t', In (t, t') ϕ <-> Some t = read_snd ϕ t') as RR'.
+  { ii; split; ii. exploit PRE; ii; des; eauto. apply read_snd_in; assumption. }
+  clear PRE.
+  induction p; ii; ss;
+  destruct p'; split; ii; ss; repeat des_hyp; clarify;
+  repeat des_goal; clarify;
+  repeat match goal with
+  | H : read_snd _ _ = _ |- _ => symmetry in H
+  | H : read_fst _ _ = _ |- _ => symmetry in H
+  | H : pmap_snd _ _ = _ |- _ => symmetry in H
+  | H : pmap_fst _ _ = _ |- _ => symmetry in H
+  end;
+  try match goal with
+  | H : Some _ = read_fst _ _ |- _ =>
+    rewrite <- RR in H; rewrite RR' in *;
+    rewrite <- H in *
+  | H : Some _ = read_snd _ _ |- _ =>
+    rewrite <- RR' in H; rewrite RR in *;
+    rewrite <- H in *
+  end; clarify;
+  match goal with
+  | H : _ = pmap_snd _ ?p |- _ =>
+    first [
+      rewrite <- IHp in H |
+      assert (Some p = Some p) as RR'' by reflexivity;
+      rewrite IHp in RR''; rewrite <- RR'' in *]; clarify
+  end.
+Qed.
+
+Definition trans_iso_C_pre `{Eq TT} `{Eq aTT} `{TotalOrder T} `{Eq aT}
+  (α' : TT -> aTT) (α : T -> aT) (φ : aTT -> aT) (φ' : aT -> aTT) (ϕ : list (TT * T))
+  (C' : dy_ctx TT) (Cout : dy_ctx T) (Cin : dy_ctx aT) :=
+  iso (Ctx (trans_C α' C')) []
+      (Ctx (trans_C α Cout [| Cin |])) [] 
+      φ φ' /\
+  (forall p (VALp : valid_path (Ctx Cout) [] p),
+    match pmap_snd ϕ p with
+    | Some p' => valid_path (Ctx C') [] p'
+    | None => False
+    end)
+.
+
+Definition trans_iso_C_post `{Eq TT} `{Eq aTT} `{TotalOrder T} `{Eq aT}
+  (α' : TT -> aTT) (inv_α : (T * aT) -> T) (α : T -> aT)
+  (φ : aTT -> aT) (φ' : aT -> aTT) (ϕ : list (TT * T)) (t : T)
+  (C' : dy_ctx TT) (Cout : dy_ctx T) (Cin : dy_ctx aT) :=
+  match trans_iso_C inv_α C' ϕ t Cout Cin with
+  | Some (C, ϕ', t') =>
+    (exists Cin', C = (Cout [|Cin'|])) /\
+    (trans_C α Cout [|Cin|]) = trans_C α C /\
+    (exists ϕ'', ϕ' = ϕ'' ++ ϕ /\
+      forall t (IN : None <> read_fst ϕ'' t),
+        reachable (Ctx C') [] t) /\
+    ϕ_spec α' α φ φ' ϕ' t' /\
+    (forall p (VALp : valid_path (Ctx C) [] p),
+      match pmap_snd ϕ' p with
+      | Some p' => valid_path (Ctx C') [] p'
+      | None => False
+      end) /\
+    (forall p' (VALp' : valid_path (Ctx C') [] p'),
+      match pmap_fst ϕ' p' with
+      | Some p => valid_path (Ctx C) [] p
+      | None => False
+      end)
+  | None => False
+  end.
+
+Definition trans_root {T aT} (α : T -> aT) (r : root T) :=
+  match r with
+  | Ctx C => Ctx (trans_C α C)
+  | Ptr t => Ptr (α t)
+  end.
+
+Lemma avp_then_vp `{Eq T} `{Eq aT} (α : T -> aT) :
+  forall p' r (VALp : valid_path (trans_root α r) [] p'),
+  exists p, valid_path r [] p /\ p' = pmap α p.
+Proof.
+  induction p'; ii; ss; repeat des_hyp; des; clarify.
+  - exists Pnil. ss.
+  - destruct r; ss; clarify.
+    rewrite trans_C_addr in *.
+    des_hyp; clarify.
+    exploit (IHp' (Ptr t)); eauto.
+    ii; des.
+    exists (Px x t p). ss. repeat rw. eauto.
+  - destruct r; ss; clarify.
+    rewrite trans_C_ctx_M in *.
+    des_hyp; clarify.
+    exploit (IHp' (Ctx d0)); eauto.
+    ii; des.
+    exists (PM M p). ss. repeat rw. eauto.
+Qed.
+
+Lemma vp_then_avp_empty `{Eq T} `{Eq aT} (α : T -> aT) :
+  forall p r (VALp : valid_path r [] p),
+  valid_path (trans_root α r) [] (pmap α p).
+Proof.
+  induction p; ii; ss; repeat des_hyp; des; clarify; ss.
+  - rewrite trans_C_addr. rw.
+    exploit IHp; eauto.
+  - rewrite trans_C_ctx_M. rw.
+    exploit IHp; eauto.
+Qed.
+
+Lemma vp_then_avp `{Eq T} `{Eq aT} (α : T -> aT) :
+  forall p r m (VALp : valid_path r m p),
+  avalid_path (trans_root α r) (trans_m α m) (pmap α p).
+Proof.
+  induction p; ii; ss; repeat des_hyp; des; clarify; ss.
+  - rewrite trans_C_addr. rw.
+    exploit IHp; eauto.
+  - rewrite trans_C_ctx_M. rw.
+    exploit IHp; eauto.
+  - des_hyp; des; clarify;
+    match goal with
+    | _ : Some ?v = read _ _ |- _ =>
+      exists (trans_v α v); s;
+      rewrite trans_m_aread
+    end.
+    all:split; try exists t; eexists; eauto.
+    all:exploit IHp; eauto.
+Qed.
+
+Lemma avp_unique `{Eq T} `{Eq aT} (α : T -> aT) :
+  forall (p p' : path T) r (VALp : valid_path r [] p)
+    (VALp' : valid_path r [] p')
+    (EQ : pmap α p = pmap α p'),
+  p = p'.
+Proof.
+  induction p; ii; destruct p';
+  ss; repeat des_hyp; des; clarify;
+  exploit IHp; eauto; ii; rw; exact eq_refl.
+Qed.
+
+Lemma pmap_fst_sound `{Eq TT} `{Eq aTT} `{TotalOrder T} `{Eq aT}
+  (α' : TT -> aTT) (α : T -> aT) (φ : aTT -> aT) (φ' : aT -> aTT) :
+  forall p p'
+    (ϕ : list (TT * T)) (t : T) (SPECϕ : ϕ_spec α' α φ φ' ϕ t)
+    (TRANS : Some p = pmap_fst ϕ p'),
+  pmap α' p' = pmap φ' (pmap α p).
+Proof.
+  induction p; ii; destruct p'; ss;
+  repeat des_hyp; des; clarify;
+  exploit IHp; eauto; ii; rrw; eauto.
+  match goal with
+  | H : read_fst _ _ = _ |- _ =>
+    symmetry in H;
+    apply read_fst_in in H as HH
+  end.
+  exploit SPECϕ; eauto.
+  ii. des. rw. eauto.
+Qed.
+
+Lemma pmap_snd_sound `{Eq TT} `{Eq aTT} `{TotalOrder T} `{Eq aT}
+  (α' : TT -> aTT) (α : T -> aT) (φ : aTT -> aT) (φ' : aT -> aTT) :
+  forall p p'
+    (ϕ : list (TT * T)) (t : T) (SPECϕ : ϕ_spec α' α φ φ' ϕ t)
+    (TRANS : Some p' = pmap_snd ϕ p),
+  pmap α p = pmap φ (pmap α' p').
+Proof.
+  induction p; ii; destruct p'; ss;
+  repeat des_hyp; des; clarify;
+  exploit IHp; eauto; ii; rrw; eauto.
+  match goal with
+  | H : read_snd _ _ = _ |- _ =>
+    symmetry in H;
+    apply read_snd_in in H as HH
+  end.
+  exploit SPECϕ; eauto.
+  ii. des. rrw. eauto.
+Qed.
+
+Lemma pmap_fst_app `{Eq TT} `{Eq aTT} `{TotalOrder T} `{Eq aT}
+  (α' : TT -> aTT) (α : T -> aT) (φ : aTT -> aT) (φ' : aT -> aTT) :
+  forall p p'
+    (ϕ ϕ' : list (TT * T)) (t t' : T)
+    (SPECϕ : ϕ_spec α' α φ φ' ϕ t)
+    (SPECϕ' : ϕ_spec α' α φ φ' (ϕ' ++ ϕ) t')
+    (TRANS : pmap_fst ϕ p = Some p'),
+  pmap_fst (ϕ' ++ ϕ) p = Some p'.
+Proof.
+  induction p; ii; ss; repeat des_hyp; des; clarify;
+  try match goal with
+  | H : read_fst _ ?tx = Some ?t |- _ =>
+    symmetry in H;
+    apply read_fst_in in H as HH;
+    exploit (SPECϕ' tx t); auto;
+    try rewrite in_app_iff; auto;
+    ii; des; rrw
+  end;
+  exploit IHp;
+  first [exact SPECϕ | eauto];
+  ii; rw; reflexivity.
+Qed.
+
+Lemma pmap_snd_app `{Eq TT} `{Eq aTT} `{TotalOrder T} `{Eq aT}
+  (α' : TT -> aTT) (α : T -> aT) (φ : aTT -> aT) (φ' : aT -> aTT) :
+  forall p p'
+    (ϕ ϕ' : list (TT * T)) (t t' : T)
+    (SPECϕ : ϕ_spec α' α φ φ' ϕ t)
+    (SPECϕ' : ϕ_spec α' α φ φ' (ϕ' ++ ϕ) t')
+    (TRANS : pmap_snd ϕ p = Some p'),
+  pmap_snd (ϕ' ++ ϕ) p = Some p'.
+Proof.
+  induction p; ii; ss; repeat des_hyp; des; clarify;
+  try match goal with
+  | H : read_snd _ ?tx = Some ?t |- _ =>
+    symmetry in H;
+    apply read_snd_in in H as HH;
+    exploit (SPECϕ' t tx); auto;
+    try rewrite in_app_iff; auto;
+    ii; des; rrw
+  end;
+  exploit IHp;
+  first [exact SPECϕ | eauto];
+  ii; rw; reflexivity.
+Qed.
+
+Lemma trans_iso_C_pre_post `{Eq TT} `{Eq aTT} `{TotalOrder T} `{Eq aT}
+  (α' : TT -> aTT) (inv_α : (T * aT) -> T) (α : T -> aT) 
+  (SPECα : inv_α_spec α inv_α) (φ : aTT -> aT) (φ' : aT -> aTT) :
+  forall (Cin : dy_ctx aT) (Cout : dy_ctx T) (C' : dy_ctx TT)
+    (ϕ : list (TT * T)) (t : T)
+    (SPECϕ : ϕ_spec α' α φ φ' ϕ t)
+    (PRE : trans_iso_C_pre α' α φ φ' ϕ C' Cout Cin),
+    trans_iso_C_post α' inv_α α φ φ' ϕ t C' Cout Cin.
+Proof.
+  induction Cin; ii;
+  unfold trans_iso_C_pre in *;
+  unfold trans_iso_C_post in *;
+  ss; des.
+  - rewrite capp_nil_r in *.
+    split. exists ([||]). rewrite capp_nil_r. eauto.
+    split. eauto.
+    split. exists []. split; eauto. ii; contradict.
+    split. eauto.
+    split. eauto.
+    destruct PRE as [PRE PRE'].
+    ii. specialize (PRE (pmap α' p')).
+    exploit PRE. apply (vp_then_avp_empty α' p' (Ctx C')). eauto.
+    ii; ss; des.
+    match goal with H : _ |- _ =>
+      apply (avp_then_vp α _ (Ctx Cout)) in H;
+      destruct H as [p'' [? RR]]
+    end. rewrite RR in *.
+    exploit PRE0; eauto. ii; des_hyp; clarify.
+    symmetry in HDES.
+    rewrite <- pmap_ϕ_bij in *.
+    assert (pmap α' p = pmap α' p').
+    { rrw. eapply pmap_fst_sound; eauto. }
+    assert (p = p').
+    { eapply (@avp_unique TT _ aTT _); eauto. }
+    clarify. rrw. eauto.
+    ii. exploit SPECϕ; eauto. ii; des; eauto.
+  - des_goal.
+    all:cycle 1.
+    (* Contradictory *)
+    des_hyp.
+    (* shadowed *)
+    exploit (IHCin (Cout [|dy_binde x (inv_α (t, tx)) ([||])|]) C' _ _ _); eauto.
+    rewrite trans_C_inject. ss.
+    destruct (SPECα t tx). rrw.
+    rewrite inject_assoc. ss. split. eauto.
+    ii. apply PRE0.
+    destruct p; ss;
+    first [rewrite inject_addr_x in *
+    | rewrite inject_ctx_M in *];
+    repeat des_hyp; des; clarify;
+    rewrite eqb_ID_eq in *; clarify.
+    rw. eauto.
+    (* not shadowed *)
+    destruct PRE as [PRE' PRE].
+    specialize (PRE (Px x tx Pnil)) as HINT.
+    exploit HINT; ss.
+    rewrite inject_addr_x.
+    rewrite trans_C_addr. rw. ss.
+    rewrite ID_refl. eauto.
+    rewrite trans_C_addr. clear HINT.
+    ii; des_hyp; des; clarify.
+    des_hyp; clarify.
+    des_hyp;
+    match goal with
+    | _ : context [(?t', inv_α (?t, ?tx))],
+      _ : read_fst _ _ = None |- _ =>
+      assert (ϕ_spec α' α φ φ' ((t', inv_α (t, tx)) :: ϕ) (inv_α (t, tx))) as SPECϕ'
+    | _ => idtac
+    end;
+    match goal with
+    | |- ϕ_spec _ _ _ _ _ _ => idtac
+    | H : trans_iso_C _ ?C' ?phi ?t ?Cout _ = None |- _ =>
+      exploit (IHCin Cout C' phi t);
+      first [rw; eauto | assumption | idtac]
+    end;
+    try rewrite trans_C_inject; s;
+    try rewrite inject_assoc; s.
+    (* addr is already inside ϕ *)
+    assert (α t1 = φ (α' t0)).
+    {
+      symmetry in HDES0.
+      apply read_fst_in in HDES0.
+      exploit SPECϕ; eauto. ii; des. eauto.
+    }
+    rw. rw. rw. 
+    split. split; eauto.
+    ii. destruct p; ss;
+    first [rewrite inject_addr_x in *
+      | rewrite inject_ctx_M in *];
+    repeat des_hyp; des; clarify.
+    exploit (PRE0 (Px x0 t2 p)). ss. rw. eauto.
+    ii. ss.
+    rewrite eqb_ID_eq in *; clarify.
+    symmetry in HDES0. apply read_fst_in in HDES0 as HH.
+    exploit SPECϕ; eauto.
+    ii; des. rrw.
+    destruct p; ss; des; clarify. rw. eauto.
+    exploit (PRE0 (PM M p)); ss; rw; eauto.
+    (* proof of ϕ_spec *)
+    ii. ss. des; clarify.
+    repeat rewrite t_refl.
+    repeat split; eauto using leb_refl.
+    destruct (SPECα t tx). rrw. rw. eauto.
+    destruct (SPECα t tx). rrw. eauto.
+    assert (eqb t'' t0 = false).
+    {
+      refl_bool. i. rewrite eqb_eq in *. clarify.
+      exploit SPECϕ; eauto. ii. des. rewrite HDES0 in *.
+      clarify.
+    }
+    assert (eqb t' (inv_α (t, tx)) = false).
+    {
+      refl_bool. i. rewrite eqb_eq in *. clarify.
+      exploit SPECϕ; eauto. ii. des.
+      destruct (SPECα t tx) as [LT RR].
+      rewrite <- RR in *.
+      destruct LT as [LE NEQ].
+      rewrite eqb_neq in *. apply NEQ.
+      apply leb_sym; eauto.
+    }
+    rw. rw. exploit SPECϕ; eauto.
+    ii; des. repeat (split; try assumption).
+    destruct (SPECα t tx) as [[? ?] ?]. lebt t.
+    destruct (SPECα t tx). rrw.
+    (* iso again *)
+    split. split; eauto.
+    ii. destruct p; simpl in VALp;
+    first [rewrite inject_addr_x in *
+      | rewrite inject_ctx_M in * | idtac];
+    repeat des_hyp; des; clarify;
+    match goal with
+    | _ =>
+      s; rewrite t_refl; rewrite eqb_ID_eq in *;
+      destruct p; ss; des; clarify; rw; eauto
+    | |- context [pmap_snd _ ?p] =>
+      exploit (PRE0 p); first [ss; rw; eauto | idtac];
+      ii; des_hyp; clarify;
+      match goal with
+      | |- context [?a :: ?l] =>
+        replace (a :: l) with ([a] ++ l) by reflexivity
+      end;
+      erewrite (@pmap_snd_app TT _ aTT _ T _ _ aT _);
+      eauto; first [exact SPECϕ | exact SPECϕ']
+    end.
+    (* now the non-contradictory cases *)
+    des_hyp.
+    (* shadowed *)
+    exploit (IHCin (Cout [|dy_binde x (inv_α (t, tx)) ([||])|]) C' _ _ _); eauto.
+    rewrite trans_C_inject. ss.
+    destruct (SPECα t tx). rrw.
+    rewrite inject_assoc. ss. split. eauto.
+    ii. apply PRE0.
+    destruct p0; ss;
+    first [rewrite inject_addr_x in *
+    | rewrite inject_ctx_M in *];
+    repeat des_hyp; des; clarify;
+    rewrite eqb_ID_eq in *; clarify.
+    rw. ii. repeat des_hyp; des; clarify.
+    rewrite trans_C_inject in *. ss.
+    rewrite inject_assoc in *. ss.
+    split. exists (dy_binde x (inv_α (t, tx)) Cin'). eauto.
+    split. rewrite trans_C_inject in *. ss.
+    destruct (SPECα t tx). rewrite <- H5 in *.
+    rewrite inject_assoc in *. ss.
+    split. exists ϕ''. eauto. eauto.
+    (* not shadowed *)
+    des_hyp; clarify.
+    destruct PRE as [PRE' PRE].
+    specialize (PRE (Px x tx Pnil)) as HINT.
+    exploit HINT; ss.
+    rewrite inject_addr_x.
+    rewrite trans_C_addr. rw. s.
+    rewrite ID_refl. eauto. clear HINT.
+    rewrite trans_C_addr. rw.
+    ii. des; clarify.
+    des_hyp;
+    match goal with
+    | _ : read_fst _ _ = None |- _ =>
+      assert (ϕ_spec α' α φ φ' ((t0, inv_α (t, tx)) :: ϕ) (inv_α (t, tx))) as SPECϕ'
+    | _ => idtac
+    end;
+    match goal with
+    | |- ϕ_spec _ _ _ _ _ _ => idtac
+    | H : trans_iso_C _ ?C' ?phi ?t ?Cout _ = _ |- _ =>
+      exploit (IHCin Cout C' phi t);
+      first [rw; eauto | assumption | idtac]
+    end;
+    try rewrite trans_C_inject; s;
+    try rewrite inject_assoc; s.
+    (* in ϕ *)
+    assert (α t1 = φ (α' t0)).
+    {
+      symmetry in HDES1.
+      apply read_fst_in in HDES1.
+      exploit SPECϕ; eauto. ii; des. eauto.
+    }
+    rw. rewrite <- x1. rw. 
+    split. split; eauto.
+    ii. destruct p0; ss;
+    first [rewrite inject_addr_x in *
+      | rewrite inject_ctx_M in *];
+    repeat des_hyp; des; clarify.
+    exploit (PRE0 (Px x0 t2 p0)). ss. rw. eauto.
+    ii. ss.
+    rewrite eqb_ID_eq in *; clarify.
+    symmetry in HDES1. apply read_fst_in in HDES1 as HH.
+    exploit SPECϕ; eauto.
+    ii; des. rrw.
+    destruct p0; ss; des; clarify. rw. eauto.
+    exploit (PRE0 (PM M p0)); ss; rw; eauto.
+    all:cycle 1.
+    (* prove ϕ_spec *)
+    ii. ss. des; clarify.
+    repeat rewrite t_refl.
+    repeat split; eauto using leb_refl.
+    destruct (SPECα t tx). rrw. rrw. eauto.
+    destruct (SPECα t tx). rrw. eauto.
+    assert (eqb t'' t0 = false).
+    {
+      refl_bool. i. rewrite eqb_eq in *. clarify.
+      exploit SPECϕ; eauto. ii. des. rewrite HDES1 in *.
+      clarify.
+    }
+    assert (eqb t' (inv_α (t, tx)) = false).
+    {
+      refl_bool. i. rewrite eqb_eq in *. clarify.
+      exploit SPECϕ; eauto. ii. des.
+      destruct (SPECα t tx) as [LT RR].
+      rewrite <- RR in *.
+      destruct LT as [LE NEQ].
+      rewrite eqb_neq in *. apply NEQ.
+      apply leb_sym; eauto.
+    }
+    rw. rw. exploit SPECϕ; eauto.
+    ii; des. repeat (split; try assumption).
+    destruct (SPECα t tx) as [[? ?] ?]. lebt t.
+    (* iso when not in ϕ *)
+    destruct (SPECα t tx). rrw.
+    split. split; eauto.
+    ii. destruct p0; simpl in VALp;
+    first [rewrite inject_addr_x in *
+      | rewrite inject_ctx_M in * | idtac];
+    repeat des_hyp; des; clarify;
+    match goal with
+    | _ =>
+      s; rewrite t_refl; rewrite eqb_ID_eq in *;
+      destruct p0; ss; des; clarify; rw; eauto
+    | |- context [pmap_snd _ ?p] =>
+      exploit (PRE0 p); first [ss; rw; eauto | idtac];
+      ii; des_hyp; clarify;
+      match goal with
+      | |- context [?a :: ?l] =>
+        replace (a :: l) with ([a] ++ l) by reflexivity
+      end;
+      erewrite (@pmap_snd_app TT _ aTT _ T _ _ aT _);
+      eauto; first [exact SPECϕ | exact SPECϕ']
+    end.
+    (* main proofs *)
+    + ii. repeat des_hyp; des; clarify.
+      repeat rewrite trans_C_inject in *.
+      repeat rewrite inject_assoc in *. ss.
+      split. eauto.
+      split. destruct (SPECα t tx) as [? RR]. rewrite <- RR in *. eauto.
+      split. exists (ϕ'' ++ [(t0, inv_α (t, tx))]).
+      rewrite <- app_assoc. s. split; eauto.
+      ii. rewrite read_fst_top in *. ss.
+      repeat des_hyp; clarify.
+      match goal with H : _ |- _ => apply H; rw; eauto end.
+      rewrite eqb_eq in *. clarify.
+      exists (Px x t0 Pnil). ss. rw. eauto.
+      eauto.
+    + ii. repeat des_hyp; des; clarify.
+      repeat rewrite trans_C_inject in *.
+      repeat rewrite inject_assoc in *. ss.
+      split. eauto.
+      split.
+      assert (φ (α' t0) = α t1).
+      {
+        symmetry in HDES1.
+        apply read_fst_in in HDES1.
+        exploit SPECϕ; eauto. ii; des. eauto.
+      }
+      assert (tx = α t1).
+      { rrw. rrw. rw. reflexivity. }
+      rw. eauto.
+      split; eauto.
+  - des_goal.
+    all:cycle 1.
+    (* Contradictory *)
+    des_hyp.
+    (* shadowed *)
+    exploit (IHCin2 (Cout [|dy_bindm M (lift_C inv_α t Cin1) ([||])|]) C' _ _ _); eauto.
+    rewrite trans_C_inject. ss.
+    rewrite lift_C_lower; eauto.
+    rewrite inject_assoc. ss. split. eauto.
+    ii. apply PRE0.
+    destruct p; ss;
+    first [rewrite inject_addr_x in *
+    | rewrite inject_ctx_M in *];
+    repeat des_hyp; des; clarify;
+    rewrite eqb_ID_eq in *; clarify.
+    rw. eauto.
+    (* not shadowed *)
+    destruct PRE as [PRE' PRE].
+    specialize (PRE (PM M Pnil)) as HINT.
+    exploit HINT; ss.
+    rewrite inject_ctx_M.
+    rewrite trans_C_ctx_M. rw. ss.
+    rewrite ID_refl. eauto.
+    rewrite trans_C_ctx_M. clear HINT.
+    ii; des_hyp; des; clarify.
+    des_hyp; clarify.
+    repeat des_hyp; clarify;
+    match goal with
+    | IHC : context [match trans_iso_C _ _ _ _ _ ?Cin with _ => _ end],
+      _ : trans_iso_C _ ?C' ?phi ?t ?Cout ?Cin = None |- _ =>
+      match goal with
+      | IHC : context [match trans_iso_C _ _ _ _ _ ?Cin with _ => _ end],
+        _ : trans_iso_C _ ?C' ?phi ?t ?Cout ?Cin = Some _ |- _ =>
+        exploit (IHC Cout C' phi t);
+        first [rw; eauto | assumption | idtac]
+      | _ =>
+        exploit (IHC Cout C' phi t);
+        first [rw; eauto | assumption | idtac]
+      end
+    end;
+    try match goal with
+    | |- context [iso] =>
+      s; split; try solve [ii; destruct p; ss];
+      split; ii;
+      match goal with
+      | _ =>
+        exploit (PRE' (PM M p)); s;
+        first [solve [rewrite trans_C_ctx_M; rw; eauto] |
+          rewrite inject_ctx_M; rewrite trans_C_ctx_M;
+          rw; s; rewrite ID_refl; subst p']
+      | _ =>
+        exploit (PRE (PM M p')); s;
+        first [solve [rewrite inject_ctx_M; rewrite trans_C_ctx_M;
+          rw; s; rewrite ID_refl; eauto] |
+          rewrite trans_C_ctx_M; rw; subst p]
+      end
+    end; ii; des; clarify.
+    ss.
+    match goal with
+    | IHC : context [match trans_iso_C _ _ _ _ _ ?Cin with _ => _ end],
+      _ : trans_iso_C _ ?C' ?phi ?t ?Cout ?Cin = None |- _ =>
+      exploit (IHC Cout C' phi t);
+      first [rw; eauto | assumption | idtac]
+    end. clear IHCin1 IHCin2.
+    rewrite trans_C_inject. s. rrw.
+    rewrite inject_assoc. s.
+    split. split; assumption.
+    ii. destruct p; ss;
+    first [rewrite inject_addr_x in *
+      | rewrite inject_ctx_M in *];
+    repeat des_hyp; des; clarify.
+    exploit (PRE0 (Px x t1 p)). s. rw. eauto.
+    ii. repeat des_hyp; clarify.
+    eapply (@pmap_snd_app TT _ aTT) with (ϕ' := ϕ'') in HDES2 as RR; eauto.
+    clear HDES2. ss. rw. eauto.
+    exploit (PRE0 (PM M0 p)). s. rw. eauto.
+    ii. repeat des_hyp; clarify.
+    eapply (@pmap_snd_app TT _ aTT) in HDES2 as RR; eauto.
+    clear HDES2. ss. rw. eauto.
+    rewrite eqb_ID_eq in *; clarify.
+    exploit x6; eauto. ii.
+    des_hyp; clarify. s. rw. eauto.
+    (* now the non-contradictory cases *)
+    des_hyp.
+    (* shadowed *)
+    match goal with
+    | IHC : context [match trans_iso_C _ _ _ _ _ ?Cin with _ => _ end],
+      _ : trans_iso_C _ ?C' ?phi ?t ?Cout ?Cin = Some _ |- _ =>
+      exploit (IHC Cout C' phi t); 
+      first [rw | assumption | idtac]
+    end;
+    ii; repeat des_hyp; des; clarify;
+    repeat rewrite trans_C_inject in *; ss;
+    rewrite lift_C_lower in *; eauto;
+    repeat rewrite inject_assoc in *; ss.
+    split. assumption.
+    ii. apply PRE0.
+    destruct p0; ss;
+    first [rewrite inject_addr_x in *
+      | rewrite inject_ctx_M in *];
+    repeat des_hyp; des; clarify.
+    rewrite eqb_ID_eq in *; clarify.
+    repeat (split; eauto).
+    (* not shadowed *)
+    destruct PRE as [PRE' PRE].
+    specialize (PRE (PM M Pnil)) as HINT.
+    exploit HINT; ss.
+    rewrite inject_ctx_M.
+    rewrite trans_C_ctx_M. rw. ss.
+    rewrite ID_refl. eauto.
+    rewrite trans_C_ctx_M. clear HINT.
+    ii; des_hyp; des; clarify.
+    des_hyp; clarify.
+    repeat des_hyp; clarify.
+    exploit (IHCin1 ([||]) d0 ϕ t); eauto; clear IHCin1.
+    match goal with
+    | |- context [iso] =>
+      s; split; try solve [ii; destruct p0; ss];
+      split; ii;
+      match goal with
+      | p : path aTT |- _ =>
+        exploit (PRE' (PM M p)); s;
+        first [solve [rewrite trans_C_ctx_M; rw; eauto] |
+          rewrite inject_ctx_M; rewrite trans_C_ctx_M;
+          rw; s; rewrite ID_refl]
+      | p' : path aT |- _ =>
+        exploit (PRE (PM M p')); s;
+        first [solve [rewrite inject_ctx_M; rewrite trans_C_ctx_M;
+          rw; s; rewrite ID_refl; eauto] |
+          rewrite trans_C_ctx_M; rw]
+      end
+    end; ii; des; clarify.
+    rw. ii. des. clarify.
+    match goal with
+    | IHC : context [match trans_iso_C _ _ _ _ _ ?Cin with _ => _ end],
+      _ : trans_iso_C _ ?C' ?phi ?t ?Cout ?Cin = Some _ |- _ =>
+      exploit (IHC Cout C' phi t); 
+      first [rw | assumption | idtac]
+    end;
+    ii; repeat des_hyp; des; clarify;
+    repeat rewrite trans_C_inject in *; ss;
+    repeat rewrite inject_assoc in *; ss; repeat rrw.
+    split. split; eauto.
+    ii. destruct p0; ss;
+    first [rewrite inject_addr_x in *
+      | rewrite inject_ctx_M in *];
+    repeat des_hyp; des; clarify.
+    exploit (PRE0 (Px x t1 p0)). s. rw. eauto.
+    ii. repeat des_hyp; clarify.
+    eapply (@pmap_snd_app TT _ aTT) with (ϕ' := ϕ'') in HDES2 as RR; eauto.
+    clear HDES2. ss. rw. eauto.
+    exploit (PRE0 (PM M0 p0)). s. rw. eauto.
+    ii. repeat des_hyp; clarify.
+    eapply (@pmap_snd_app TT _ aTT) in HDES2 as RR; eauto.
+    clear HDES2. ss. rw. eauto.
+    rewrite eqb_ID_eq in *; clarify.
+    exploit x6; eauto. ii.
+    des_hyp; clarify. s. rw. eauto.
+    (* finish off *)
+    repeat (split; eauto).
+    rewrite app_assoc. eexists. split. reflexivity.
+    ii. rewrite read_fst_top in *.
+    repeat des_hyp. 
+    match goal with H : _ |- _ => apply H; rw; eauto end.
+    assert (reachable (Ctx d0) [] t2) as HINT. eauto.
+    unfold reachable in HINT. des.
+    exists (PM M p). s. rw. eauto.
+Qed.
+
+Fixpoint find_iso `{Eq aTT} `{Eq aT}
+  (v : expr_value aTT) (vl : list (expr_value aT)) φ φ' :=
+  match vl with
+  | [] => None
+  | v' :: vl' =>
+    match v, v' with
+    | Closure e C, Closure e' C' =>
+      if eq_val e e' && iso_C C C' φ φ'
+      then Some v'
+      else find_iso v vl' φ φ'
+    end
+  end.
+
+Fixpoint remove_t `{Eq T} (m : memory T) t :=
+  match m with
+  | [] => []
+  | (t', v) :: tl =>
+    let tl := remove_t tl t in
+    if eqb t t' then tl else (t', v) :: tl
+  end.
+
+Lemma remove_t_dec `{Eq T} :
+  forall (m : memory T) t,
+  (List.length (remove_t m t)) <= (List.length m).
+Proof.
+  induction m; intros; simpl; eauto;
+  repeat des_goal; repeat des_hyp; clarify;
+  try rewrite eqb_eq in *; subst;
+  match goal with
+  | |- context [remove_t _ ?t] =>
+    specialize (IHm t); nia
+  end.
+Qed.
+
+Lemma remove_t_strict_dec `{Eq T} :
+  forall (m : memory T) t (READ : None <> read m t),
+  (List.length (remove_t m t)) < (List.length m).
+Proof.
+  induction m; intros; simpl; eauto; clarify.
+  des_goal. rewrite eqb_comm.
+  repeat des_goal; repeat des_hyp; clarify;
+  try rewrite eqb_eq in *; subst.
+  pose proof (remove_t_dec m t). nia.
+  ss.
+  revert READ. rw. ii. exploit IHm; eauto.
+  nia.
+Qed.
+
+Lemma remove_t_read `{Eq T} :
+  forall (m : memory T) t,
+  None = read (remove_t m t) t.
+Proof.
+  induction m; ii; ss; repeat des_goal; repeat des_hyp; clarify.
+  rewrite eqb_eq in *; clarify. rewrite t_refl in *. clarify.
+Qed.
+
+Lemma remove_t_read_some `{Eq T} :
+  forall (m : memory T) t t' (NEQ : t <> t'),
+  read (remove_t m t) t' = read m t'.
+Proof.
+  induction m; ii; ss; repeat des_goal; repeat des_hyp;
+  try rewrite eqb_eq in *; clarify; eauto.
+Qed.
+
+Lemma vpath_less_then_vpath_more `{Eq T} :
+  forall a b p r (VAL : valid_path r a p),
+  valid_path r (a ++ b) p.
+Proof.
+  ii.
+  ginduction p; ii; ss;
+  repeat des_hyp; des; clarify; eauto.
+  des_hyp; des; clarify.
+  all:match goal with
+  | RR : Some ?v = read _ _ |- _ =>
+    exists v; rewrite read_top; rewrite <- RR; eauto
+  end.
+Qed.
+
+Lemma avpath_less_then_avpath_more `{Eq T} :
+  forall a b p r (VAL : avalid_path r a p),
+  avalid_path r (a ++ b) p.
+Proof.
+  ii.
+  ginduction p; ii; ss;
+  repeat des_hyp; des; clarify; eauto.
+  des_hyp; des; clarify.
+  all:match goal with
+  | RR : In ?v (aread _ _) |- _ =>
+    exists v; rewrite aread_in in *;
+    rewrite in_app_iff; eauto
+  end.
+Qed.
+
+Lemma avpath_trans_empty `{Eq T} `{Eq TT} (φ : T -> TT) :
+  forall p C C' m' (VAL : avalid_path (Ctx C) [] p)
+    (VAL' : avalid_path (Ctx C') m' (pmap φ p)),
+  avalid_path (Ctx C') [] (pmap φ p).
+Proof.
+  induction p; ii; ss; repeat des_hyp; des; clarify.
+  - destruct p; ss; des; clarify.
+  - eapply IHp; eauto.
+Qed.
+
+Fixpoint plen {T} (p : path T) :=
+  match p with
+  | Pnil => 0
+  | PM _ p
+  | Pv _ p
+  | Px _ _ p => S (plen p)
+  end.
+
+Inductive trans_res T TT :=
+  | Unchanged
+  | Changed (t : T) (v : expr_value T)
+            (t' : TT) (v' : expr_value TT) 
+            (ϕ : list (T * TT)) (tϕ : TT)
+  | Failed
+.
+
+Arguments Unchanged {T TT}.
+Arguments Changed {T TT}.
+Arguments Failed {T TT}.
+
+Fixpoint trans_m_step `{Eq TT} `{Eq aTT} `{TotalOrder T} `{Eq aT}
+  (α' : TT -> aTT) (inv_α : (T * aT) -> T) φ φ'
+  (ϕ : list (TT * T)) (tϕ : T)
+  (m : memory aT) (m' : memory TT) :=
+  match m' with
+  | [] => Unchanged
+  | (t', v') :: tl' =>
+    match read_fst ϕ t' with
+    | None => trans_m_step α' inv_α φ φ' ϕ tϕ m tl'
+    | Some t =>
+      match v' with
+      | Closure e' C' =>
+      match find_iso (trans_v α' v') (aread m (φ (α' t'))) φ φ' with
+      | None => Failed
+      | Some (Closure e C) =>
+        match trans_iso_C inv_α C' ϕ tϕ ([||]) C with
+        | None => Failed
+        | Some (C, ϕ, tϕ) =>
+          Changed t' v' t (Closure e C) ϕ tϕ
+        end
+      end end
+    end
+  end.
+
+Definition trans_m_step_pre `{Eq TT} `{Eq aTT} `{TotalOrder T} `{Eq aT}
+  (α' : TT -> aTT) φ φ' 
+  (ϕ : list (TT * T)) (m : memory aT) (m' : memory TT) :=
+  forall t' (IN : None <> read_fst ϕ t'),
+    match read m' t' with
+    | None => True
+    | Some v' =>
+      exists v, In v (aread m (φ (α' t'))) /\
+      match (trans_v α' v'), v with
+      | Closure e' C', Closure e C =>
+        e' = e /\ iso (Ctx C') [] (Ctx C) [] φ φ'
+      end
+    end.
+
+Definition trans_m_step_post `{Eq TT} `{Eq aTT} `{TotalOrder T} `{Eq aT}
+  (α' : TT -> aTT) (inv_α : (T * aT) -> T) (α : T -> aT) φ φ'
+  (ϕ : list (TT * T)) (tϕ : T)
+  (m : memory aT) (m' : memory TT) :=
+  match trans_m_step α' inv_α φ φ' ϕ tϕ m m' with
+  | Unchanged =>
+    forall t' (IN : None <> read_fst ϕ t'),
+      None = read m' t'
+  | Changed t' (Closure e' C') t (Closure e C) ϕ_af tϕ_af =>
+    Some t = read_fst ϕ t' /\ e' = e /\
+    Some (Closure e' C') = read m' t' /\
+    In (Closure e (trans_C α C)) (aread m (α t)) /\
+    ϕ_spec α' α φ φ' ϕ_af tϕ_af /\
+    (exists ϕ', ϕ_af = ϕ' ++ ϕ /\
+      forall t' (IN : None <> read_fst ϕ' t'),
+        reachable (Ctx C') [] t') /\
+    (forall p (VALp : valid_path (Ctx C) [] p),
+      match pmap_snd ϕ_af p with
+      | Some p' => valid_path (Ctx C') [] p'
+      | None => False
+      end) /\
+    (forall p' (VALp' : valid_path (Ctx C') [] p'),
+      match pmap_fst ϕ_af p' with
+      | Some p => valid_path (Ctx C) [] p
+      | None => False
+      end)
+  | Failed => False
+  end.
+
+Lemma find_iso_spec `{Eq aTT} `{Eq aT} φ φ' :
+  forall (vl : list (expr_value aT)) (v' : expr_value aTT)
+  (PRE : exists v, In v vl /\
+    match v', v with
+    | Closure e' C', Closure e C =>
+      e' = e /\ iso (Ctx C') [] (Ctx C) [] φ φ'
+    end),
+  exists v, Some v = find_iso v' vl φ φ' /\
+    In v vl /\
+    match v', v with
+    | Closure e' C', Closure e C =>
+      e' = e /\ iso (Ctx C') [] (Ctx C) [] φ φ'
+    end.
+Proof.
+  induction vl; ii; des; repeat des_hyp; clarify.
+  ss; des; clarify.
+  - rewrite <- check_iso_iso in *. rw.
+    solve_eqb eq_val. rewrite t_refl. s.
+    eexists. split. reflexivity.
+    rewrite check_iso_iso in *.
+    eauto.
+  - repeat des_goal; repeat des_hyp.
+    rewrite eq_val_eq in *;
+    rewrite check_iso_iso in *; clarify.
+    eexists. split. reflexivity. s. eauto.
+    all:(exploit IHvl);
+    first [solve[
+      eexists; split; eauto;
+      instantiate (1 := Closure e0 C); s; eauto] |
+      ii; des; eauto].
+Qed.
+
+Lemma trans_m_step_pre_post `{Eq TT} `{Eq aTT} `{TotalOrder T} `{Eq aT}
+  (α' : TT -> aTT) (inv_α : (T * aT) -> T) (α : T -> aT) 
+  (SPECα : inv_α_spec α inv_α) φ φ' :
+  forall (m' : memory TT) (m : memory aT)
+    (ϕ : list (TT * T)) (tϕ : T)
+    (SPECϕ : ϕ_spec α' α φ φ' ϕ tϕ)
+    (PRE : trans_m_step_pre α' φ φ' ϕ m m'),
+  trans_m_step_post α' inv_α α φ φ' ϕ tϕ m m'.
+Proof.
+  induction m'; ii; ss.
+  destruct a as [t' v'].
+  destruct (read_fst ϕ t') eqn:CASE;
+  red; s; rw.
+  - exploit (PRE t'). rw. ii; clarify.
+    s. rewrite t_refl. intros [v [INv ISOv]].
+    exploit (find_iso_spec φ φ' (aread m (φ (α' t'))) (trans_v α' v')); eauto.
+    intros [v'' [RR ISOv'']]. rrw. clear RR.
+    destruct v' as [e' C'].
+    destruct v'' as [e'' C''].
+    ss; repeat des_hyp; des; clarify.
+    exploit (trans_iso_C_pre_post α' inv_α α SPECα φ φ' C'' ([||]) C' ϕ tϕ SPECϕ).
+    split. s. eauto.
+    ii; ss. destruct p; ss.
+    intros POST. unfold trans_iso_C_post in POST.
+    repeat des_hyp; clarify.
+    rewrite t_refl. des; clarify.
+    repeat (split; eauto).
+    exploit (SPECϕ t' t).
+    symmetry in CASE. apply read_fst_in in CASE. eauto.
+    ii. des. rw. eauto.
+  - assert (trans_m_step_pre α' φ φ' ϕ m m') as PRE'.
+    {
+      ii. exploit PRE; eauto.
+      s. des_goal; des_hyp.
+      rewrite eqb_eq in *. clarify. contradict.
+      rw. eauto. rw. eauto.
+    }
+    exploit IHm'; eauto.
+    intros POST. unfold trans_m_step_post in POST.
+    des_hyp; clarify.
+    ii. des_goal; eauto.
+    rewrite eqb_eq in *. clarify. contradict.
+    repeat des_hyp; des; clarify.
+    assert (eqb t' t = false).
+    {
+      rewrite eqb_neq. ii. clarify. rewrite CASE in *. clarify.
+    }
+    rw. repeat (split; eauto).
+Qed.
+
+Lemma reachable_disj `{Eq T} :
+  forall r m m' t (REACH : reachable r m t)
+    (DISJ : forall t (READ : None <> read m t), None = read m' t),
+  reachable r (m' ++ m) t.
+Proof.
+  ii. destruct REACH as [p [VALp INp]].
+  ginduction p; ii; ss;
+  repeat des_hyp; des; clarify.
+  - exists (Px x t0 Pnil). s. rw. eauto.
+  - exploit IHp; eauto. intros [p' [VALp' INp']].
+    exists (Px x t0 p'). s. rw. eauto.
+  - exploit IHp; eauto. intros [p' [VALp' INp']].
+    exists (PM M p'). s. rw. eauto.
+  - des_hyp; des; clarify.
+    exploit IHp; eauto. intros [p' [VALp' INp']].
+    exists (Pv e p').
+    s. split; eauto. exists (Closure e C).
+    rewrite read_top.
+    exploit (DISJ t0). rrw; ii; clarify.
+    ii. rrw. eauto.
+Qed.
+
+Lemma paste_vpath `{Eq T} :
+  forall r m t t' (REACH : reachable r m t)
+    (REACH' : reachable (Ptr t) m t'),
+  reachable r m t'.
+Proof.
+  ii. destruct REACH as [p [VALp INp]].
+  ginduction p; ii; ss;
+  repeat des_hyp; des; clarify.
+  - destruct REACH' as [p' [VALp' INp']].
+    exists (Px x t0 p'). s. rw. eauto.
+  - exploit IHp; eauto. intros [p' [VALp' INp']].
+    exists (Px x t0 p'). s. rw. eauto.
+  - exploit IHp; eauto. intros [p' [VALp' INp']].
+    exists (PM M p'). s. rw. eauto.
+  - des_hyp; des; clarify.
+    exploit IHp; eauto. intros [p' [VALp' INp']].
+    exists (Pv e p'). s. split; eauto.
+    exists (Closure e C). eauto.
+Qed.
+
+Lemma tail_vpath `{Eq T} :
+  forall r m t (REACH : reachable r m t),
+    reachable r [] t \/
+    exists t' e C,
+      (r = Ptr t' \/ reachable r m t') /\
+      Some (Closure e C) = read m t' /\
+      reachable (Ctx C) [] t.
+Proof.
+  intros. destruct REACH as [p [VALp INp]].
+  ginduction p; ii; ss;
+  repeat des_hyp; des; clarify.
+  - left. exists (Px x t0 Pnil). s. rw. eauto.
+  - exploit IHp; eauto.
+    intros REACH'; des.
+    destruct REACH' as [p' [? ?]].
+    destruct p'; ss; des; clarify.
+    clarify.
+    right. exists t'. exists e. exists C0.
+    repeat (split; try assumption). right.
+    exists (Px x t' Pnil). s. rw. eauto.
+    right. exists t'. exists e. exists C0.
+    repeat (split; try assumption). right.
+    eapply paste_vpath; eauto.
+    exists (Px x t0 Pnil). s. rw. eauto.
+  - exploit IHp; eauto.
+    intros REACH'; des; clarify;
+    destruct REACH' as [p' [? ?]].
+    left. exists (PM M p'). s. rw. eauto.
+    right. exists t'. exists e. exists C0.
+    repeat (split; try assumption). right.
+    exists (PM M p'). s. rw. eauto.
+  - des_hyp; des; clarify. right.
+    exploit IHp; eauto.
+    intros REACH'; des; clarify;
+    destruct REACH' as [p' [? ?]].
+    exists t0. exists e. exists C.
+    repeat (split; eauto). exists p'. eauto.
+    exists t'. exists e0. exists C0.
+    repeat (split; try assumption). right.
+    exists (Pv e p').
+    s. split; eauto.
+    exists (Closure e C). eauto.
+Qed.
+
+Definition equiv_fst_ϕ_m `{Eq T} `{Eq TT} (ϕ : list (T * TT)) m m' :=
+  forall t p e C
+  (READ : Some (Closure e C) = read m t)
+  (VALp : valid_path (Ctx C) [] p),
+  match read_fst ϕ t with
+  | Some t' =>
+    match pmap_fst ϕ p with
+    | Some p' =>
+      exists C', Some (Closure e C') = read m' t' /\
+        valid_path (Ctx C') [] p'
+    | None => False
+    end 
+  | None => False
+  end.
+
+Definition equiv_snd_ϕ_m `{Eq T} `{Eq TT} (ϕ : list (T * TT)) m m' :=
+  forall t p e C
+  (READ : Some (Closure e C) = read m t)
+  (VALp : valid_path (Ctx C) [] p),
+  match read_snd ϕ t with
+  | Some t' =>
+    match pmap_snd ϕ p with
+    | Some p' =>
+      exists C', Some (Closure e C') = read m' t' /\
+        valid_path (Ctx C') [] p'
+    | None => False
+    end 
+  | None => False
+  end.
+
+Definition equiv_fst_ϕ_C `{Eq T} `{Eq TT} (ϕ : list (T * TT)) C C' :=
+  forall p
+    (VALp : valid_path (Ctx C) [] p),
+  match pmap_fst ϕ p with
+  | Some p' => valid_path (Ctx C') [] p'
+  | None => False
+  end.
+
+Definition equiv_snd_ϕ_C `{Eq T} `{Eq TT} (ϕ : list (T * TT)) C C' :=
+  forall p
+    (VALp : valid_path (Ctx C) [] p),
+  match pmap_snd ϕ p with
+  | Some p' => valid_path (Ctx C') [] p'
+  | None => False
+  end.
+
+Lemma equiv_fst_ϕ_aux `{Eq T} `{Eq TT} (ϕ : list (T * TT)) 
+  m m' (EQm : equiv_fst_ϕ_m ϕ m m') :
+  forall n C C' (EQC : equiv_fst_ϕ_C ϕ C C')
+    p (VALp : valid_path (Ctx C) m p)
+    (LE : plen p <= n),
+  match pmap_fst ϕ p with
+  | Some p' => valid_path (Ctx C') m' p'
+  | None => False
+  end.
+Proof.
+  unfold equiv_fst_ϕ_m in *.
+  unfold equiv_fst_ϕ_C in *.
+  induction n.
+  ii. destruct p; ss; nia.
+  ii; ss. destruct p; ss.
+  - des_hyp; des; clarify.
+    exploit (EQC (Px x t Pnil)). s. rw. eauto.
+    s. ii. repeat des_hyp; des; clarify.
+    ss. des_hyp; des; clarify.
+    destruct n; ss.
+    destruct p; ss; first [rw; eauto | nia].
+    destruct p; ss. rw. eauto.
+    des. des_hyp; des; clarify.
+    exploit (EQm t Pnil _ _ _); eauto.
+    ii. repeat des_hyp; des; clarify.
+    exploit (IHn C0 C'0 _ p); eauto.
+    ii.
+    exploit (EQm t p0); eauto. repeat rw.
+    ii. repeat des_hyp; des; clarify.
+    revert x2. rrw. ii. clarify. nia.
+    ii. des_hyp.
+    s. rw. split; eauto. eexists. split; eauto. s. eauto.
+  - des_hyp.
+    exploit (EQC (PM M Pnil)). s. rw. eauto.
+    ii. ss. des_hyp.
+    exploit (IHn d d0 _ p).
+    ii. exploit (EQC (PM M p0)). s. rw. eauto.
+    s. ii. repeat des_hyp; clarify.
+    revert x1. s. rw. eauto. eauto. nia.
+    ii. des_hyp. s. rw. eauto.
+Qed.
+
+Lemma equiv_snd_ϕ_aux `{Eq T} `{Eq TT} (ϕ : list (T * TT)) 
+  m m' (EQm : equiv_snd_ϕ_m ϕ m m') :
+  forall n C C' (EQC : equiv_snd_ϕ_C ϕ C C')
+    p (VALp : valid_path (Ctx C) m p)
+    (LE : plen p <= n),
+  match pmap_snd ϕ p with
+  | Some p' => valid_path (Ctx C') m' p'
+  | None => False
+  end.
+Proof.
+  unfold equiv_snd_ϕ_m in *.
+  unfold equiv_snd_ϕ_C in *.
+  induction n.
+  ii. destruct p; ss; nia.
+  ii; ss. destruct p; ss.
+  - des_hyp; des; clarify.
+    exploit (EQC (Px x t Pnil)). s. rw. eauto.
+    s. ii. repeat des_hyp; des; clarify.
+    ss. des_hyp; des; clarify.
+    destruct n; ss.
+    destruct p; ss; first [rw; eauto | nia].
+    destruct p; ss. rw. eauto.
+    des. des_hyp; des; clarify.
+    exploit (EQm t Pnil _ _ _); eauto.
+    ii. repeat des_hyp; des; clarify.
+    exploit (IHn C0 C'0 _ p); eauto.
+    ii.
+    exploit (EQm t p0); eauto. repeat rw.
+    ii. repeat des_hyp; des; clarify.
+    revert x2. rrw. ii. clarify. nia.
+    ii. des_hyp.
+    s. rw. split; eauto. eexists. split; eauto. s. eauto.
+  - des_hyp.
+    exploit (EQC (PM M Pnil)). s. rw. eauto.
+    ii. ss. des_hyp.
+    exploit (IHn d d0 _ p).
+    ii. exploit (EQC (PM M p0)). s. rw. eauto.
+    s. ii. repeat des_hyp; clarify.
+    revert x1. s. rw. eauto. eauto. nia.
+    ii. des_hyp. s. rw. eauto.
+Qed.
+
+Inductive fix_result `{Eq T} `{Eq TT} :=
+  | Fix (m mbot : memory T) (m' : memory TT) (ϕ : list (T * TT)) (tϕ : TT)
+  | Unfix
+.
+
+Fixpoint trans_iso_m_aux `{Eq TT} `{Eq aTT} `{TotalOrder T} `{Eq aT}
+  (α' : TT -> aTT) (inv_α : (T * aT) -> T) φ φ'
+  (ϕ : list (TT * T)) (tϕ : T)
+  (am : memory aT) (m1 : memory T) (m2 m : memory TT) fuel :=
+  match trans_m_step α' inv_α φ φ' ϕ tϕ am m with
+  | Unchanged => Fix m2 m m1 ϕ tϕ
+  | Changed t' v' t v ϕ' tϕ' =>
+    let m1' := (t, v) :: m1 in
+    let m2' := (t', v') :: m2 in
+    let m' := remove_t m t' in
+    match fuel with
+    | 0 => Unfix
+    | S fuel' => trans_iso_m_aux α' inv_α φ φ' ϕ' tϕ' am m1' m2' m' fuel'
+    end
+  | Failed => Unfix
+  end.
+
+Definition trans_iso_m `{Eq TT} `{Eq aTT} `{TotalOrder T} `{Eq aT}
+  (α' : TT -> aTT) (inv_α : (T * aT) -> T) φ φ'
+  (ϕ : list (TT * T)) (tϕ : T)
+  (am : memory aT) (m : memory TT) :=
+  trans_iso_m_aux α' inv_α φ φ' ϕ tϕ am [] [] m (length m).
+
+Definition trans_iso_m_pre `{Eq TT} `{Eq aTT} `{TotalOrder T} `{Eq aT}
+  (α' : TT -> aTT) (inv_α : (T * aT) -> T) (α : T -> aT) φ φ'
+  (ϕ : list (TT * T)) (tϕ : T) (C2 : dy_ctx TT) (C1 : dy_ctx T)
+  (am : memory aT) (m1 : memory T) (m2 m : memory TT) :=
+  (forall t, None <> read m2 t -> None = read m t) /\
+  (forall t, reachable (Ctx C2) m2 t <-> None <> read_fst ϕ t) /\
+  equiv_fst_ϕ_C ϕ C2 C1 /\
+  equiv_snd_ϕ_C ϕ C1 C2 /\
+  equiv_fst_ϕ_m ϕ m2 m1 /\
+  equiv_snd_ϕ_m ϕ m1 m2 /\
+  ϕ_spec α' α φ φ' ϕ tϕ /\
+  inv_α_spec α inv_α /\
+  aIso (Ctx (trans_C α' C2)) (trans_m α' (m2 ++ m))
+       (Ctx (trans_C α C1)) am φ φ' /\
+  (forall t v, Some v = read m1 t ->
+    In (trans_v α v) (aread am (α t)))
+.
+
+Lemma pre_implies_pre `{Eq TT} `{Eq aTT} `{TotalOrder T} `{Eq aT}
+  (α' : TT -> aTT) (inv_α : (T * aT) -> T) (α : T -> aT) φ φ'
+  (ϕ : list (TT * T)) (tϕ : T) (C2 : dy_ctx TT) (C1 : dy_ctx T)
+  (am : memory aT) (m1 : memory T) (m2 m : memory TT) :
+  trans_iso_m_pre α' inv_α α φ φ' ϕ tϕ C2 C1 am m1 m2 m ->
+  trans_m_step_pre α' φ φ' ϕ am m.
+Proof.
+  intros ISO.
+  ii. unfold trans_iso_m_pre in ISO. des.
+  assert (reachable (Ctx C2) m2 t') as REACH.
+  { rewrite <- ISO0 in *. assumption. }
+  unfold aIso in *.
+  des_goal; eauto.
+  des.
+  assert (areachable (Ctx (trans_C α' C2)) (trans_m α' (m2 ++ m)) (α' t')).
+  {
+    destruct REACH as [p [VALp INp]].
+    apply vpath_less_then_vpath_more with (b := m) in VALp.
+    apply vp_then_avp with (α := α') in VALp.
+    exists (pmap α' p). split; eauto.
+    clear IN GDES VALp.
+    generalize dependent t'.
+    induction p; ii; ss; des; clarify; eauto.
+  }
+  exploit (ISO9 _ (trans_v α' e)); eauto.
+  {
+    rewrite trans_m_aread.
+    rewrite <- disj_reflect in ISO.
+    exploit (ISO t'). rw. ii; clarify. ii.
+    exists t'. exists e. rewrite read_top. rrw. eauto.
+  }
+  ii; des. exists v'. split; eauto.
+  repeat des_hyp; des; clarify.
+  rewrite <- check_aiso_aiso in *.
+  rewrite <- iso_C_is_aiso_C in *.
+  rewrite check_iso_iso in *. eauto.
+Qed.
+
+Lemma pmap_fst_read `{Eq T} `{Eq TT} (ϕ: list (T * TT)) :
+  forall p p' t (MAP : pmap_fst ϕ p = Some p') (IN : Inp t p),
+  None <> read_fst ϕ t.
+Proof.
+  induction p; ii; ss; repeat des_hyp; des; clarify.
+  all:try solve [exploit IHp; eauto].
+  rewrite HDES in *. clarify.
+Qed.
+
+Lemma pmap_snd_read `{Eq T} `{Eq TT} (ϕ: list (T * TT)) :
+  forall p p' t (MAP : pmap_snd ϕ p = Some p') (IN : Inp t p),
+  None <> read_snd ϕ t.
+Proof.
+  induction p; ii; ss; repeat des_hyp; des; clarify.
+  all:try solve [exploit IHp; eauto].
+  rewrite HDES in *. clarify.
+Qed.
+
+Lemma same_valid `{Eq T} :
+  forall p r m1 m2 (SAME : same m1 m2),
+    valid_path r m1 p <-> valid_path r m2 p.
+Proof.
+  induction p; ii; ss; split; ii; repeat des_hyp; des; clarify.
+  rw; eauto. unfold same in *. ii. rw. eauto.
+  rw; eauto. rw; eauto. unfold same in *; ii; rw; eauto.
+  rw; eauto.
+  des_hyp; des; clarify. unfold same in SAME. rewrite SAME in *.
+  eexists. split; eauto. s. rw; eauto. ii. rw. eauto.
+  des_hyp; des; clarify. unfold same in SAME. rewrite <- SAME in *.
+  eexists. split; eauto. s. rw; eauto.
+Qed.
+
+Lemma asame_avalid `{Eq T} :
+  forall p r m1 m2 (SAME : asame m1 m2),
+    avalid_path r m1 p <-> avalid_path r m2 p.
+Proof.
+  induction p; ii; ss; split; ii; repeat des_hyp; des; clarify.
+  rw; eauto. unfold asame in *. ii. rw. eauto.
+  rw; eauto. rw; eauto. unfold asame in *; ii; rw; eauto.
+  rw; eauto.
+  des_hyp; des; clarify. unfold asame in SAME. rewrite SAME in *.
+  eexists. split; eauto. s. rw; eauto. ii. rw. eauto.
+  des_hyp; des; clarify. unfold asame in SAME. rewrite <- SAME in *.
+  eexists. split; eauto. s. rw; eauto.
+Qed.
+
+Lemma asame_aIso `{Eq T} `{Eq TT} (φ : T -> TT) φ' :
+  forall r m1 m2 r' m' (SAME : asame m1 m2) (ISO : aIso r m2 r' m' φ φ'),
+  aIso r m1 r' m' φ φ'.
+Proof.
+  ii. destruct ISO as [[ISO ISO'] [ISO'' ISO''']]. ss.
+  split. split; ss.
+  ii. apply ISO. rewrite asame_avalid in *; eauto.
+  split; ii; ss.
+  ii. rewrite asame_avalid; eauto.
+  split; ii. destruct REACH as [p [VALp INp]].
+  apply ISO''. exists p. split; eauto. rewrite <- asame_avalid; eauto.
+  unfold asame in SAME. rewrite <- SAME. eauto.
+  exploit ISO'''; eauto. ii; des.
+  exists v.
+  unfold asame in *. rewrite SAME. eauto.
+Qed.
+
+Lemma trans_m_iso_pre_post `{Eq TT} `{Eq aTT} `{TotalOrder T} `{Eq aT}
+  n (α' : TT -> aTT) (inv_α : (T * aT) -> T) (α : T -> aT) φ φ'
+  (ϕ : list (TT * T)) (tϕ : T) (C2 : dy_ctx TT) (C1 : dy_ctx T)
+  (am : memory aT) (m1 : memory T) (m2 m : memory TT)
+  (LE : length m <= n)
+  (PRE : trans_iso_m_pre α' inv_α α φ φ' ϕ tϕ C2 C1 am m1 m2 m) :
+  match trans_iso_m_aux α' inv_α φ φ' ϕ tϕ am m1 m2 m n with
+  | Fix m2' m' m1' ϕ' tϕ' =>
+    (trans_iso_m_pre α' inv_α α φ φ' ϕ' tϕ' C2 C1 am m1' m2' m') /\
+    same (m2 ++ m) (m2' ++ m') /\
+    (forall t' (IN : None <> read_fst ϕ' t'), None = read m' t')
+  | Unfix => False
+  end.
+Proof.
+  ginduction n; ii; ss.
+  destruct m; ss; nia.
+  apply pre_implies_pre in PRE as PRE'.
+  unfold trans_iso_m_pre in PRE. des.
+  exploit (@trans_m_step_pre_post TT _ aTT _ T _ _ aT); eauto.
+  intros POST. unfold trans_m_step_post in *.
+  repeat des_hyp; eauto.
+  repeat (split; eauto).
+  des; clarify.
+  assert (read m2 t = None) as DISJ.
+  {
+    destruct (read m2 t) eqn:CASE; eauto.
+    exploit (PRE t). rw. ii; clarify.
+    repeat rrw. ii; clarify.
+  }
+  assert (same ((t, Closure e0 C) :: m2 ++ remove_t m t) (m2 ++ m)) as SAME.
+  {
+    apply same_trans with (m' := m2 ++ ([(t, Closure e0 C)] ++ remove_t m t)).
+    rewrite app_assoc.
+    match goal with
+    | |- context [?a :: ?b ++ ?c] =>
+      replace (a :: b ++ c) with (([a] ++ b) ++ c) by reflexivity
+    end.
+    apply app_same.
+    apply app_disj_same. ii; ss. des_hyp; clarify.
+    rewrite eqb_eq in *. clarify.
+    split; ii; ss.
+    apply app_same. split; ii; ss.
+    split; ii; ss.
+    repeat des_hyp; clarify. rewrite eqb_eq in *. clarify.
+    rewrite remove_t_read_some in *; eauto. rewrite eqb_neq in *. eauto.
+    des_goal. rewrite eqb_eq in *. clarify. repeat rw. eauto.
+    rewrite remove_t_read_some; eauto. rewrite eqb_neq in *. eauto.
+  }
+  exploit (IHn TT _ aTT _ T _ _ aT _ α' inv_α α φ φ' (ϕ' ++ ϕ) tϕ0 C2 C1 am ((t', Closure e0 C0) :: m1) ((t, Closure e0 C) :: m2) (remove_t m t)); eauto.
+  exploit (remove_t_strict_dec m t).
+  repeat rrw. rw. ii; clarify. nia.
+  split. ii; ss. des_hyp. rewrite eqb_eq in *; clarify.
+  erewrite remove_t_read; eauto.
+  exploit PRE; eauto. erewrite remove_t_read_some; eauto.
+  rewrite <- eqb_neq. eauto.
+  repeat match goal with |- _ /\ _ => split end.
+  - ii. split; intros REACH. apply tail_vpath in REACH.
+    des; clarify.
+    destruct REACH as [p [VALp INp]].
+    apply vpath_less_then_vpath_more with (b := m2) in VALp; ss.
+    assert (None <> read_fst ϕ t0). rewrite <- PRE0. exists p. eauto.
+    rewrite read_fst_top.
+    repeat des_goal; clarify.
+    destruct (eqb t t'0) eqn:CASE.
+    rewrite eqb_eq in *. clarify. ss. rewrite t_refl in *. clarify.
+    destruct REACH1 as [p [VALp INp]].
+    exploit POST6; eauto.
+    des_goal; clarify.
+    ii. exploit (pmap_fst_read (ϕ' ++ ϕ) p); eauto.
+    ss. rewrite CASE in *. destruct REACH1 as [p [VALp INp]].
+    exploit PRE3; eauto.
+    ii. repeat des_hyp; des; clarify.
+    exploit (pmap_fst_read ϕ p); eauto.
+    rewrite read_fst_top in *. repeat des_hyp; clarify.
+    assert (reachable (Ctx C2) m2 t) as REACH'.
+    { rewrite PRE0. rrw. ii; clarify. }
+    rewrite read_fst_top in *. repeat des_hyp; clarify.
+    exploit (POST7 t0). rw. ii; clarify. intros [p [VALp INp]].
+    apply paste_vpath with (t := t).
+    apply reachable_disj with (m' := [(t, Closure e0 C)]); eauto.
+    rewrite <- disj_reflect. ii; ss.
+    des_hyp; clarify. rewrite eqb_eq in *; clarify.
+    exists (Pv e0 p). s. split; eauto.
+    rewrite t_refl. eexists. split; eauto.
+    s. split; eauto.
+    exploit (vpath_less_then_vpath_more [] _ p (Ctx C)); eauto.
+    rewrite <- PRE0 in REACH.
+    apply reachable_disj with (m' := [(t, Closure e0 C)]); eauto.
+    rewrite <- disj_reflect. ii; ss.
+    des_hyp; clarify. rewrite eqb_eq in *; clarify.
+  - ii. exploit PRE1; eauto. ii. des_hyp.
+    erewrite (@pmap_fst_app TT _ aTT _ T _ _ aT); eauto.
+  - ii. exploit PRE2; eauto. ii. des_hyp.
+    erewrite (@pmap_snd_app TT _ aTT _ T _ _ aT); eauto.
+  - ii; ss. des_hyp; clarify.
+    rewrite eqb_eq in *. clarify. exploit POST6; eauto.
+    assert (read_fst (ϕ' ++ ϕ) t0 = Some t').
+    {
+      apply read_fst_in in POST.
+      exploit (POST3 t0 t'). rewrite in_app_iff; eauto.
+      ii. des. rrw. eauto.
+    }
+    rw. ii. des_hyp. rewrite t_refl. eexists. split; eauto.
+    exploit PRE3; eauto.
+    ii. repeat des_hyp; des; clarify.
+    assert (read_fst (ϕ' ++ ϕ) t0 = Some t1).
+    {
+      symmetry in HDES1.
+      apply read_fst_in in HDES1.
+      exploit (POST3 t0 t1). rewrite in_app_iff; eauto.
+      ii. des. rrw. eauto.
+    }
+    rw. erewrite (@pmap_fst_app TT _ aTT _ T _ _ aT); eauto.
+    assert (eqb t' t1 = false).
+    {
+      rewrite eqb_neq. ii. clarify.
+      apply read_fst_in in POST.
+      exploit (PRE5 t t1); eauto. ii; des.
+      symmetry in HDES1. apply read_fst_in in HDES1.
+      exploit (PRE5 t0 t1); eauto. ii; des.
+      rewrite <- x3 in *. clarify. rewrite t_refl in *. clarify.
+    }
+    rw. eexists. split; eauto.
+  - ii; ss. des_hyp; clarify.
+    rewrite eqb_eq in *. clarify. exploit POST5; eauto.
+    assert (read_snd (ϕ' ++ ϕ) t0 = Some t).
+    {
+      apply read_fst_in in POST.
+      exploit (POST3 t t0). rewrite in_app_iff; eauto.
+      ii. des. rrw. eauto.
+    }
+    rw. ii. des_hyp. rewrite t_refl. eexists. split; eauto.
+    exploit PRE4; eauto.
+    ii. repeat des_hyp; des; clarify.
+    assert (read_snd (ϕ' ++ ϕ) t0 = Some t1).
+    {
+      symmetry in HDES1.
+      apply read_snd_in in HDES1.
+      exploit (POST3 t1 t0). rewrite in_app_iff; eauto.
+      ii. des. rrw. eauto.
+    }
+    rw. erewrite (@pmap_snd_app TT _ aTT _ T _ _ aT); eauto.
+    assert (eqb t t1 = false).
+    {
+      rewrite eqb_neq. ii. clarify.
+      apply read_fst_in in POST.
+      exploit (PRE5 t1 t'); eauto. ii; des.
+      symmetry in HDES1. apply read_snd_in in HDES1.
+      exploit (PRE5 t1 t0); eauto. ii; des.
+      rewrite <- x2 in *. clarify. rewrite t_refl in *. clarify.
+    }
+    rw. eexists. split; eauto.
+  - eauto.
+  - eauto.
+  - eapply asame_aIso with (m2 := trans_m α' (m2 ++ m)); eauto.
+    apply trans_m_asame; eauto.
+  - ii; ss. des_hyp; eauto.
+    rewrite eqb_eq in *. clarify.
+  - ii. des_hyp; des. split; eauto. split; eauto.
+    eapply same_trans; eauto.
+    rewrite same_comm. eauto.
+Qed.
+
+Lemma separate_mem `{Eq T} (P : T -> Prop) :
+  forall p r m1 m2 
+    (M1 : forall t, (r = Ptr t \/ reachable r m1 t) -> P t)
+    (M2 : forall t, P t -> read m2 t = None)
+    (VAL : valid_path r (m1 ++ m2) p),
+  valid_path r m1 p.
+Proof.
+  induction p; ii; ss;
+  repeat des_hyp; des; clarify.
+  - split; eauto. eapply IHp; eauto.
+    intros t' [? | [p' [VALp INp]]]; clarify; apply M1; right.
+    exists (Px x t' Pnil). s. rw. eauto.
+    exists (Px x t p'). s. rw. eauto.
+  - eapply IHp; eauto.
+    intros ? [? | [p' [VALp INp]]]; clarify; apply M1; right.
+    exists (PM M p'). s. rw. eauto.
+  - des_hyp; des; clarify.
+    assert (P t).
+    apply M1. eauto.
+    exploit M2; eauto. ii.
+    rewrite read_top in *.
+    repeat des_hyp; clarify.
+    eexists. split; eauto. s. split; eauto.
+    eapply IHp; eauto.
+    intros t' [? | [p' [VALp INp]]]; clarify; apply M1; right.
+    exists (Pv e p'). s. split; eauto.
+    eexists. split; eauto. s. eauto.
+    rewrite <- VAL in *. clarify.
+Qed.
+
+Fixpoint lift_m `{TotalOrder T} `{Eq aT}
+  (inv_α : (T * aT) -> T) (t : T) (m : memory aT) :=
+  match m with
+  | [] => []
+  | (t', Closure e C) :: m' =>
+    let t' := inv_α (t, t') in
+    (t', Closure e (lift_C inv_α t C)) ::
+    lift_m inv_α t' m'
+  end.
+
+Lemma lift_m_lower_aux `{TotalOrder T} `{Eq aT} 
+  (α : T -> aT) (inv_α : (T * aT) -> T) (SPECα : inv_α_spec α inv_α) :
+  forall m t seen (LE : forall t', In t' seen -> leb t' t = true),
+  trans_m_aux α (lift_m inv_α t m) seen = m.
+Proof.
+  induction m; ii; ss.
+  repeat des_goal; clarify.
+  - rewrite Inb_eq in *.
+    exploit LE; eauto.
+    specialize (SPECα t a0). des.
+    rewrite <- not_le_lt in *.
+    rewrite SPECα. ii; clarify.
+  - specialize (SPECα t a0) as RR. des.
+    rrw. rewrite lift_C_lower; eauto.
+    rewrite IHm. reflexivity.
+    ii; ss; des; clarify. solve_leb.
+    lebt t. eauto. apply RR.
+Qed.
+
+Lemma lift_m_lower `{TotalOrder T} `{Eq aT} 
+  (α : T -> aT) (inv_α : (T * aT) -> T) (SPECα : inv_α_spec α inv_α) :
+  forall m t, trans_m α (lift_m inv_α t m) = m.
+Proof.
+  ii. apply lift_m_lower_aux; eauto.
+Qed.
+
+Lemma lift_m_disj `{TotalOrder T} `{Eq aT}
+  (α : T -> aT) (inv_α : (T * aT) -> T) (SPECα : inv_α_spec α inv_α) :
+  forall m t t', None <> read (lift_m inv_α t m) t' -> t << t'.
+Proof.
+  induction m; ii; ss.
+  repeat des_hyp; clarify.
+  - rewrite eqb_eq in *; clarify. apply SPECα.
+  - exploit IHm; eauto.
+    intros LT. rewrite <- not_le_lt.
+    refl_bool. intros LE.
+    assert (leb t t' = true).
+    lebt (inv_α (t, a0)). apply SPECα. apply LT.
+    assert (t = t'). apply leb_sym; eauto.
+    clarify. destruct LT.
+    assert (leb t' (inv_α (t', a0)) = true).
+    apply SPECα.
+    assert (t' = inv_α (t', a0)) as RR. apply leb_sym; eauto.
+    rewrite <- RR in *. rewrite t_refl in *. clarify.
+Qed.
+
+Lemma app_disj_asame `{Eq T} `{Eq aT} (α : T -> aT) :
+  forall m m' (DISJ : forall t, None <> read m t -> None = read m' t),
+  asame (trans_m α (m ++ m')) (trans_m α m ++ trans_m α m').
+Proof.
+  ii.
+  repeat rewrite aread_in. rewrite in_app_iff.
+  repeat rewrite <- aread_in.
+  repeat rewrite trans_m_aread.
+  split; intros IN; des; clarify.
+  rewrite read_top in *.
+  des_hyp; clarify.
+  - left. eexists. eexists. repeat (split; eauto).
+  - right. eexists. eexists. repeat (split; eauto).
+  - exists t'. exists v'. rewrite read_top.
+    rrw. eauto.
+  - exists t'. exists v'. rewrite read_top.
+    rewrite disj_reflect in DISJ.
+    exploit (DISJ t'). rrw. ii; clarify.
+    ii. rrw. eauto.
+Qed.
+
+Definition trans_iso `{Eq TT} `{Eq aTT} `{TotalOrder T} `{Eq aT}
+  (α' : TT -> aTT) (inv_α : (T * aT) -> T) (init : T) φ φ'
+  (C : dy_ctx TT) (m : memory TT) (aC : dy_ctx aT) (am : memory aT) :=
+  match trans_iso_C inv_α C [] init ([||]) aC with
+  | Some (CC, ϕ, tϕ) =>
+    match trans_iso_m_aux α' inv_α φ φ' ϕ tϕ am [] [] m (length m) with
+    | Fix m2' m' m1' ϕ' tϕ' =>
+      Some (CC, m1' ++ lift_m inv_α tϕ' am, ϕ')
+    | Unfix => None
+    end
+  | None => None
+  end.
+
+Lemma trans_iso_pre_post `{Eq TT} `{Eq aTT} `{TotalOrder T} `{Eq aT}
+  (α' : TT -> aTT) (inv_α : (T * aT) -> T) (α : T -> aT) (SPECα : inv_α_spec α inv_α)
+  (init : T) φ φ' (C : dy_ctx TT) (m : memory TT) 
+  (aC : dy_ctx aT) (am : memory aT) 
+  (ISO : aIso (Ctx (trans_C α' C)) (trans_m α' m) (Ctx aC) am φ φ') :
+  match trans_iso α' inv_α init φ φ' C m aC am with
+  | Some (CC, mm, ϕ) =>
+    (forall t t' (IN : In (t, t') ϕ),
+      Some t' = read_fst ϕ t /\
+      Some t = read_snd ϕ t') /\
+    trans_C α CC = aC /\
+    asame (trans_m α mm) am /\
+    (forall p (VALp : valid_path (Ctx C) m p),
+      match pmap_fst ϕ p with
+      | Some p' => valid_path (Ctx CC) mm p'
+      | None => False
+      end) /\
+    (forall p (VALp : valid_path (Ctx CC) mm p),
+      match pmap_snd ϕ p with
+      | Some p' => valid_path (Ctx C) m p'
+      | None => False
+      end)
+  | None => False
+  end.
+Proof.
+  unfold trans_iso.
+  assert (trans_iso_C_pre α' α φ φ' [] C ([||]) aC) as PREC.
+  {
+    split. s. destruct ISO as [ISO ELSE]. clear ELSE.
+    rewrite <- check_iso_iso. rewrite iso_C_is_aiso_C.
+    rewrite check_aiso_aiso.
+    destruct ISO as [ISO ISO'].
+    split; ss.
+    ii. exploit (ISO p).
+    eapply avpath_less_then_avpath_more with (a := []); eauto.
+    ii; des. exploit (avpath_trans_empty φ p); eauto.
+    ii. exploit (ISO' p').
+    eapply avpath_less_then_avpath_more with (a := []); eauto.
+    ii; des. exploit (avpath_trans_empty φ' p'); eauto.
+    ii. destruct p; ss.
+  }
+  exploit (@trans_iso_C_pre_post TT _ aTT _ T _ _ aT); eauto.
+  instantiate (1 := init). ii. ss.
+  intros POSTC.
+  unfold trans_iso_C_post in POSTC.
+  des_hyp. repeat des_hyp; des; clarify.
+  rewrite app_nil_r in *.
+  assert (trans_iso_m_pre α' inv_α α φ φ' ϕ'' t C Cin' am [] [] m) as PREm.
+  {
+    split. ii; ss. split.
+    ii. split; intros REACH; eauto.
+    destruct REACH as [p [VALp INp]].
+    exploit POSTC4; eauto. ii. des_hyp.
+    exploit (@pmap_fst_read TT _ T); eauto.
+    repeat (split; try solve [ii; ss | eauto]).
+  }
+  exploit (@trans_m_iso_pre_post TT _ aTT _ T _ _ aT); eauto.
+  intros POSTm; ss. unfold trans_iso_m_pre in POSTm.
+  des_hyp; des.
+  split. ii. exploit POSTm7; eauto. ii; des. eauto.
+  split; eauto.
+  split. eapply asame_trans. apply app_disj_asame.
+  - rewrite <- disj_reflect. ii.
+    exploit lift_m_disj; eauto. intros LT.
+    unfold equiv_snd_ϕ_m in *.
+    destruct (read m' t0) eqn:CASE; eauto.
+    destruct e as [ev Cv].
+    symmetry in CASE.
+    exploit (POSTm6 t0 Pnil ev Cv CASE); ss.
+    des_goal; ss. symmetry in GDES.
+    apply read_snd_in in GDES.
+    exploit (POSTm7 t1 t0); eauto. ii; des.
+    rewrite <- not_le_lt in *.
+    rewrite LT in *. clarify.
+  - rewrite lift_m_lower; eauto.
+    split; ii; rewrite aread_in in *;
+    rewrite in_app_iff in *; des; eauto.
+    rewrite <- aread_in in *.
+    rewrite trans_m_aread in *. des.
+    exploit POSTm10; eauto. repeat rw. eauto.
+  - split; ii.
+    erewrite same_valid in VALp; eauto.
+    exploit (separate_mem (fun t' => None <> read_fst ϕ t') p (Ctx C) m0 mbot).
+    ii; des; clarify. rewrite POSTm2 in *. eauto.
+    ii. symmetry. eauto. eauto.
+    ii.
+    exploit (@equiv_fst_ϕ_aux TT _ T); eauto.
+    des_goal; ss. ii. apply vpath_less_then_vpath_more; eauto.
+    exploit (separate_mem (fun t' => leb t' tϕ = true) p (Ctx Cin') m' (lift_m inv_α tϕ am)).
+    intros t' [? | [p' [VALp' INp']]]; clarify.
+    exploit (@equiv_snd_ϕ_aux TT _ T); eauto.
+    des_goal; ss. ii.
+    pose proof (@pmap_snd_read TT _ T _ ϕ p' p0 t' GDES INp').
+    destruct (read_snd ϕ t') eqn:READ; ss.
+    symmetry in READ. apply read_snd_in in READ.
+    exploit (POSTm7 t0 t'); eauto. ii; des. eauto.
+    ii. destruct (read (lift_m inv_α tϕ am) t0) eqn:READ; eauto.
+    exploit lift_m_disj; eauto. rw. ii; clarify. intros LT.
+    rewrite <- not_le_lt in *. rewrite LT in *. clarify. eauto.
+    ii.
+    exploit (@equiv_snd_ϕ_aux TT _ T); eauto.
+    ii. des_hyp; clarify.
+    rewrite same_valid. instantiate (1 := m0 ++ mbot).
+    apply vpath_less_then_vpath_more. eauto. eauto.
+Qed.
+
+Definition derived_fst `{Eq T} `{Eq TT} (ϕ : list (T * TT)) (init' : TT) t :=
+  match read_fst ϕ t with
+  | Some t' => t'
+  | None => init'
+  end.
+
+Definition derived_snd `{Eq T} `{Eq TT} (ϕ : list (T * TT)) (init : T) t' :=
+  match read_snd ϕ t' with
+  | Some t => t
+  | None => init
+  end.
+
+Lemma derived_fst_map `{Eq T} `{Eq TT} (ϕ : list (T * TT)) (init' : TT) :
+  forall p p' (MAP : pmap_fst ϕ p = Some p'),
+  pmap (derived_fst ϕ init') p = p'.
+Proof.
+  induction p; ii; 
+  unfold derived_fst in *; ss; repeat des_hyp; des; clarify;
+  erewrite IHp; eauto.
+Qed.
+
+Lemma derived_snd_map `{Eq T} `{Eq TT} (ϕ : list (T * TT)) (init : T) :
+  forall p p' (MAP : pmap_snd ϕ p = Some p'),
+  pmap (derived_snd ϕ init) p = p'.
+Proof.
+  induction p; ii; 
+  unfold derived_snd in *; ss; repeat des_hyp; des; clarify;
+  erewrite IHp; eauto.
+Qed.
+
+Theorem concretization_preserves_equivalence `{Eq T} `{Eq aT} `{TotalOrder TT} `{Eq aTT}
+  (α : T -> aT) (inv_α' : (TT * aTT) -> TT) (α' : TT -> aTT) (SPECα' : inv_α_spec α' inv_α')
+  (init : T) (init' : TT) φ φ' 
+  (C : dy_ctx T) (m : memory T) (aC : dy_ctx aTT) (am : memory aTT)
+  (ISO : aIso (Ctx (trans_C α C)) (trans_m α m) (Ctx aC) am φ φ') :
+  exists C' m' f f',
+    trans_C α' C' = aC /\ asame (trans_m α' m') am /\
+    iso (Ctx C) m (Ctx C') m' f f'.
+Proof.
+  exploit (@trans_iso_pre_post T _ aT _ TT _ _ aTT); eauto.
+  instantiate (1 := init').
+  intros HINT. repeat des_hyp; des.
+  exists d. exists l0. exists (derived_fst l init'). exists (derived_snd l init).
+  split; eauto. split; eauto.
+  split; ss; ii.
+  - exploit HINT2; eauto. ii; des_hyp.
+    erewrite derived_fst_map; eauto.
+    split; eauto. erewrite derived_snd_map; eauto.
+    symmetry. rewrite <- pmap_ϕ_bij; eauto.
+  - exploit HINT3; eauto. ii; des_hyp.
+    erewrite derived_snd_map; eauto.
+    split; eauto. erewrite derived_fst_map; eauto.
+    symmetry. rewrite pmap_ϕ_bij; eauto.
+Qed.
